<?xml version="1.0"?>
<rdf:RDF xmlns="http://ontology.inrae.fr/ppdo/ontology"
     xml:base="http://ontology.inrae.fr/ppdo/ontology"
     xmlns:dc="http://purl.org/dc/elements/1.1/"
     xmlns:owl="http://www.w3.org/2002/07/owl#"
     xmlns:rdf="http://www.w3.org/1999/02/22-rdf-syntax-ns#"
     xmlns:xml="http://www.w3.org/XML/1998/namespace"
     xmlns:xsd="http://www.w3.org/2001/XMLSchema#"
     xmlns:rdfs="http://www.w3.org/2000/01/rdf-schema#"
     xmlns:skos="http://www.w3.org/2004/02/skos/core#"
     xmlns:vann="http://purl.org/vocab/vann/"
     xmlns:terms="http://purl.org/dc/terms/">
    <owl:Ontology rdf:about="http://ontology.inrae.fr/ppdo/ontology">
        <owl:versionIRI rdf:resource="http://ontology.inrae.fr/ppdo/ontology/20200818"/>
        <owl:imports rdf:resource="http://www.w3.org/2004/02/skos/core"/>
        <dc:description xml:lang="fr">Ce fichier RDF contient une extension du modèle SKOS pour modeliser les stades de développement (ou stades phénologiques) des plantes cultivées. Ce modèle défini des classes représentant les stades principaux et les stades secondaires. Il a été construit pendant le projet ANR D2KAB.

Contacter Catherine Roussey (catherine.roussey@inrae.fr) pour toute modification dans ce fichier.

Ce modele skos a été construit en utilisant 4 versions de la monographie BBCH toutes sous licence  Creative Commons Attribution 4.0 International: 
* Growth stages of mono- and dicotyledonous plants BBCH Monograph edited by Uwe Meier Julius Kühn-Institut (JKI) Quedlinburg 2018 
DOI: 10.5073/20180906-074619
ISBN: 978-3-95547-071-5
* Stades phénologiques des mono-et dicotylédones cultivées BBCH
Monographie rédigé par Uwe Meier Instituto Julius Kühn (JKI, siglas en alomán) Quedlinburg, 2018 
DOI: 10.5073/20180906-075455
ISBN: 978-3-95547-072-2
* Estadios de las plantas mono-y dicotyledóneas BBCH Monografia Elaborado por Uwe Meier Instituto Julius Kühn (JKI, siglas en alomán) Quedlinburg, 2018 
DOI: 10.5073/20180906-075743
ISBN: 978-3-95547-069-2
* Entwicklungsstadien mono- und dikotyler Pflanzen BBCH Monografie bearbeitet von Uwe Meier Julius Kühn-Institut (JKI) Quedlinburg 2018 DOI: 10.5073/20180906-075119
ISBN: 978-3-95547-070-8</dc:description>
        <dc:description xml:lang="en">This RDF file contains an extension of the SKOS model to model the development stages (or phenological stages) of cultivated plants. This model defines classes representing the main stages and the secondary stages. It was built during the ANR D2KAB project.

Contact Catherine Roussey (catherine.roussey@inrae.fr) for any modification in this file.

This extension of SKOS model was build using 4 versions of BBCH monograph: 
* Growth stages of mono- and dicotyledonous plants BBCH Monograph edited by Uwe Meier Julius Kühn-Institut (JKI) Quedlinburg 2018 
DOI: 10.5073/20180906-074619
ISBN: 978-3-95547-071-5
* Stades phénologiques des mono-et dicotylédones cultivées BBCH
Monographie rédigé par Uwe Meier Instituto Julius Kühn (JKI, siglas en alomán) Quedlinburg, 2018 
DOI: 10.5073/20180906-075455
ISBN: 978-3-95547-072-2
* Estadios de las plantas mono-y dicotyledóneas BBCH Monografia Elaborado por Uwe Meier Instituto Julius Kühn (JKI, siglas en alomán) Quedlinburg, 2018 
DOI: 10.5073/20180906-075743
ISBN: 978-3-95547-069-2
* Entwicklungsstadien mono- und dikotyler Pflanzen BBCH Monografie bearbeitet von Uwe Meier Julius Kühn-Institut (JKI) Quedlinburg 2018 DOI: 10.5073/20180906-075119
ISBN: 978-3-95547-070-8
All versions are licensed under a Creative Commons Attribution 4.0 International License.</dc:description>
        <dc:issued rdf:datatype="http://www.w3.org/2001/XMLSchema#dateTime">2020-12-04T00:00:00+01:00</dc:issued>
        <dc:issued rdf:datatype="http://www.w3.org/2001/XMLSchema#dateTime">2021-03-08T00:00:00+01:00</dc:issued>
        <dc:publisher>https://www6.clermont.inrae.fr/tscf</dc:publisher>
        <dc:title xml:lang="en">model for plant phenological stages</dc:title>
        <terms:contributor xml:lang="en">Florence AMARDEILH, Elzeard, France
Sophie AUBIN, INRAE, DIPSO, France
Stephan BERNARD, INRAE, TSCF, France
Robert BOSSY, INRAE, France
Remi CERES, Elzeard, France
Xavier DELPUECH, IFV, France
Matthieu HIRSCHY, Acta, France
Clement JONQUET, LIRMM, Montpellier, France
Franck MICHEL, CNRS I3S, France
Marc RAYNAL, IFV, France</terms:contributor>
        <terms:contributor>https://orcid.org/0000-0001-6652-9319</terms:contributor>
        <terms:contributor>https://orcid.org/0000-0001-7278-3209</terms:contributor>
        <terms:contributor xml:lang="en">https://orcid.org/0000-0001-9064-0463</terms:contributor>
        <terms:contributor xml:lang="en">https://orcid.org/0000-0001-9694-1443</terms:contributor>
        <terms:contributor xml:lang="en">https://orcid.org/0000-0002-2404-1582</terms:contributor>
        <terms:contributor xml:lang="en">https://orcid.org/0000-0002-6306-4437</terms:contributor>
        <terms:contributor xml:lang="en">https://orcid.org/0000-0003-4805-8220</terms:contributor>
        <terms:creator xml:lang="en">Catherine ROUSSEY, INRAE, TSCF, France</terms:creator>
        <terms:creator>https://orcid.org/0000-0002-3076-5499</terms:creator>
        <terms:licence xml:lang="en">This work is licensed under a Creative Commons Attribution 4.0 International License.
http://creativecommons.org/licenses/by/4.0/</terms:licence>
        <vann:preferredNamespacePrefix>ppdo</vann:preferredNamespacePrefix>
        <owl:versionInfo rdf:datatype="http://www.w3.org/2001/XMLSchema#decimal">1.0</owl:versionInfo>
    </owl:Ontology>
    


    <!-- 
    ///////////////////////////////////////////////////////////////////////////////////////
    //
    // Annotation properties
    //
    ///////////////////////////////////////////////////////////////////////////////////////
     -->

    


    <!-- http://purl.org/dc/elements/1.1/description -->

    <owl:AnnotationProperty rdf:about="http://purl.org/dc/elements/1.1/description"/>
    


    <!-- http://purl.org/dc/elements/1.1/issued -->

    <owl:AnnotationProperty rdf:about="http://purl.org/dc/elements/1.1/issued"/>
    


    <!-- http://purl.org/dc/elements/1.1/modified -->

    <owl:AnnotationProperty rdf:about="http://purl.org/dc/elements/1.1/modified"/>
    


    <!-- http://purl.org/dc/elements/1.1/publisher -->

    <owl:AnnotationProperty rdf:about="http://purl.org/dc/elements/1.1/publisher"/>
    


    <!-- http://purl.org/dc/elements/1.1/title -->

    <owl:AnnotationProperty rdf:about="http://purl.org/dc/elements/1.1/title"/>
    


    <!-- http://purl.org/dc/terms/contributor -->

    <owl:AnnotationProperty rdf:about="http://purl.org/dc/terms/contributor"/>
    


    <!-- http://purl.org/dc/terms/creator -->

    <owl:AnnotationProperty rdf:about="http://purl.org/dc/terms/creator"/>
    


    <!-- http://purl.org/dc/terms/description -->

    <owl:AnnotationProperty rdf:about="http://purl.org/dc/terms/description"/>
    


    <!-- http://purl.org/dc/terms/licence -->

    <owl:AnnotationProperty rdf:about="http://purl.org/dc/terms/licence"/>
    


    <!-- http://purl.org/dc/terms/title -->

    <owl:AnnotationProperty rdf:about="http://purl.org/dc/terms/title"/>
    


    <!-- http://purl.org/vocab/vann/preferredNamespacePrefix -->

    <owl:AnnotationProperty rdf:about="http://purl.org/vocab/vann/preferredNamespacePrefix"/>
    


    <!-- 
    ///////////////////////////////////////////////////////////////////////////////////////
    //
    // Object Properties
    //
    ///////////////////////////////////////////////////////////////////////////////////////
     -->

    


    <!-- http://ontology.inrae.fr/ppdo/ontology/follows -->

    <owl:ObjectProperty rdf:about="http://ontology.inrae.fr/ppdo/ontology/follows">
        <owl:inverseOf rdf:resource="http://ontology.inrae.fr/ppdo/ontology/precedes"/>
        <rdfs:comment>propriété equivalent à IAO_0000115. Faut il créer une sous propriété pour dehja mettre une définition en francais, indiquer qu&apos;elle bne doit lier que deux stades</rdfs:comment>
    </owl:ObjectProperty>
    


    <!-- http://ontology.inrae.fr/ppdo/ontology/hasRank -->

    <owl:ObjectProperty rdf:about="http://ontology.inrae.fr/ppdo/ontology/hasRank">
        <rdfs:comment>cette proriété est uns sous property de has_quality de BFO R0_0000086</rdfs:comment>
        <skos:definition xml:lang="fr">Cette propriété lie un stade phénologique à une division:   principal ou  secondaire</skos:definition>
        <skos:definition xml:lang="en">This property links a growth stage to a division: principal  stage or secondary stage</skos:definition>
        <skos:prefLabel xml:lang="fr">a pour rang</skos:prefLabel>
        <skos:prefLabel xml:lang="en">has rank</skos:prefLabel>
    </owl:ObjectProperty>
    


    <!-- http://ontology.inrae.fr/ppdo/ontology/precedes -->

    <owl:ObjectProperty rdf:about="http://ontology.inrae.fr/ppdo/ontology/precedes">
        <skos:definition xml:lang="en">This property links a stage to the following stage</skos:definition>
        <skos:prefLabel xml:lang="en">precedes</skos:prefLabel>
        <skos:prefLabel xml:lang="fr">précède</skos:prefLabel>
    </owl:ObjectProperty>
    


    <!-- 
    ///////////////////////////////////////////////////////////////////////////////////////
    //
    // Classes
    //
    ///////////////////////////////////////////////////////////////////////////////////////
     -->

    


    <!-- http://ontology.inrae.fr/ppdo/ontology/GrowthStage -->

    <owl:Class rdf:about="http://ontology.inrae.fr/ppdo/ontology/GrowthStage">
        <rdfs:subClassOf rdf:resource="http://www.w3.org/2004/02/skos/core#Concept"/>
        <skos:altLabel xml:lang="es">estadio de crecimiento</skos:altLabel>
        <skos:altLabel xml:lang="es">etapa de desarrollo</skos:altLabel>
        <skos:altLabel xml:lang="en">phenological development stage</skos:altLabel>
        <skos:altLabel xml:lang="en">phenological stage</skos:altLabel>
        <skos:altLabel xml:lang="en">plant development stage</skos:altLabel>
        <skos:altLabel xml:lang="fr">stade phénologique</skos:altLabel>
        <skos:definition xml:lang="de">Die erweiterte BBCH-Skala zur einheitlichen Codierung der phänologischen Entwicklungsstadien mono- und dikotyler Pflanzen (Quelle BBCh monografie)</skos:definition>
        <skos:definition xml:lang="es">La escala extendida BBCH es un sistema para una codificación uniforme de identificación fenológica de estadios de crecimiento para todas las especies de plantas mono - y dicotiledóneas. (fuente BBCH monografia)</skos:definition>
        <skos:definition xml:lang="fr">codification homogène des stades phénologiques des plantes cultivées et description de ces stades. (source BBCH monographie)</skos:definition>
        <skos:definition xml:lang="en">standardised coding  of plant development stages with description of their phenological characteristics. (source BBCH monograph)</skos:definition>
        <skos:note xml:lang="es">D = Dicotiledóneas
M = Monocotiledóneas
G = Gramineas
P = Perennes
V = Desarrollo a partir de partes vegetativas o de órganos de propagación</skos:note>
        <skos:note xml:lang="en">D= Dicotyledons
M= Monocotyledons
V= Development from vegetative parts or propagated organs.
G= Gramineae
P= Perennial plants
No code letter is used if the description applies to all groups of plants.</skos:note>
        <skos:note xml:lang="fr">M = Monocotylédones
G = Graminées
D = Dicotylédones
P = Plantes pérennes
V = développement à partir d’organes végétatifs de réserve ou de multiplication

Aucun autre code n’est utilisé si la description est valable pour tous les groupes de végétaux.</skos:note>
        <skos:note xml:lang="de">M = Monokotyle 
G = Gramineen
D = Dikotyle 
P = Perennierende Pflanzen / Dauerkulturen
V= Entwicklung aus vegetativen Überdauerungs- bzw. Vermehrungsorganen
Gilt die Beschreibung für alle Pflanzengruppen, so wird diese zusätzliche Kennzeichnung weggelassen.</skos:note>
        <skos:prefLabel xml:lang="de">Entwicklungsstadium</skos:prefLabel>
        <skos:prefLabel xml:lang="es">estadio de desarrollo</skos:prefLabel>
        <skos:prefLabel xml:lang="en">growth stage</skos:prefLabel>
        <skos:prefLabel xml:lang="fr">stade de développement</skos:prefLabel>
    </owl:Class>
    


    <!-- http://ontology.inrae.fr/ppdo/ontology/PrincipalGrowthStage -->

    <owl:Class rdf:about="http://ontology.inrae.fr/ppdo/ontology/PrincipalGrowthStage">
        <owl:equivalentClass>
            <owl:Class>
                <owl:intersectionOf rdf:parseType="Collection">
                    <rdf:Description rdf:about="http://ontology.inrae.fr/ppdo/ontology/GrowthStage"/>
                    <owl:Restriction>
                        <owl:onProperty rdf:resource="http://ontology.inrae.fr/ppdo/ontology/hasRank"/>
                        <owl:hasValue rdf:resource="http://ontology.inrae.fr/ppdo/ontology/principal"/>
                    </owl:Restriction>
                </owl:intersectionOf>
            </owl:Class>
        </owl:equivalentClass>
        <rdfs:subClassOf rdf:resource="http://ontology.inrae.fr/ppdo/ontology/GrowthStage"/>
        <skos:definition xml:lang="de">Der gesamte Entwicklungszyklus der Pflanzen ist mit Ziffern in aufsteigender Reihenfolge von O bis 9 in zehn überschaubare und deutlich voneinander abgrenzbare längere Entwicklungsphasen, den Makrostadien unterteilt. (quelle BBCH monografie)</skos:definition>
        <skos:definition xml:lang="es">El ciclo completo de desarrollo de las plantas se subdivide en diez fases principales de desarrollo claramente distinguibles. Estos estadios principales de crecimiento, son descritos usando números del 0 al 9 en orden ascendente (fuente BBCH monografia).</skos:definition>
        <skos:definition xml:lang="fr">Les différentes phases du développement d’une plante sont divisées en dix stades principaux numérotés de 0 à 9. Ces différentes phases de développement sont de longue durée et clairement reconnaissables.(source BBCH monographie)</skos:definition>
        <skos:definition xml:lang="en">The entire developmental cycle of the plants is subdivided into ten clearly recognizable and distinguishable longer-lasting developmental phases. These principal growth stages are described using numbers from 0 to 9 in ascending order. (source BBCH monograph)</skos:definition>
        <skos:prefLabel xml:lang="es">estadio principale de crecimiento</skos:prefLabel>
        <skos:prefLabel xml:lang="de">makrostadium</skos:prefLabel>
        <skos:prefLabel xml:lang="en">principal growth stage</skos:prefLabel>
        <skos:prefLabel xml:lang="fr">stade de développement principal</skos:prefLabel>
    </owl:Class>
    


    <!-- http://ontology.inrae.fr/ppdo/ontology/PrincipalStage0 -->

    <owl:Class rdf:about="http://ontology.inrae.fr/ppdo/ontology/PrincipalStage0">
        <rdfs:subClassOf rdf:resource="http://ontology.inrae.fr/ppdo/ontology/PrincipalGrowthStage"/>
        <rdfs:seeAlso rdf:datatype="http://www.w3.org/2001/XMLSchema#string">http://aims.fao.org/aos/agrovoc/c_15923</rdfs:seeAlso>
        <skos:definition xml:lang="es">Germinación, brotación, desarrollo de la yema (fuente BBCH monografia)</skos:definition>
        <skos:definition xml:lang="en">Germination / sprouting / bud development (source BBCH monograph)</skos:definition>
        <skos:definition xml:lang="de">Keimung / Austrieb (Quelle BBCH Monografie)</skos:definition>
        <skos:definition xml:lang="fr">germination / levée / développement des bourgeons  (source BBCH monographie)</skos:definition>
        <skos:prefLabel xml:lang="de">Makrostadium 0</skos:prefLabel>
        <skos:prefLabel xml:lang="es">estadio principal 0</skos:prefLabel>
        <skos:prefLabel xml:lang="en">principal stage 0</skos:prefLabel>
        <skos:prefLabel xml:lang="fr">stade principal 0</skos:prefLabel>
    </owl:Class>
    


    <!-- http://ontology.inrae.fr/ppdo/ontology/PrincipalStage1 -->

    <owl:Class rdf:about="http://ontology.inrae.fr/ppdo/ontology/PrincipalStage1">
        <rdfs:subClassOf rdf:resource="http://ontology.inrae.fr/ppdo/ontology/PrincipalGrowthStage"/>
        <rdfs:seeAlso rdf:datatype="http://www.w3.org/2001/XMLSchema#string">http://aims.fao.org/aos/agrovoc/c_1af7de35</rdfs:seeAlso>
        <skos:definition xml:lang="de">Blattentwicklung (Hauptsproß) (Quelle BBCH Monografie)</skos:definition>
        <skos:definition xml:lang="es">Desarrollo de las hojas (brote o tallo principal) (fuente BBCH monografia)</skos:definition>
        <skos:definition xml:lang="en">Leaf development (main shoot) (source BBCH monograph)</skos:definition>
        <skos:definition xml:lang="fr">développement des feuilles (tige principale) (source BBCH monographie)</skos:definition>
        <skos:prefLabel xml:lang="de">Makrostadium 1</skos:prefLabel>
        <skos:prefLabel xml:lang="es">estadio principal 1</skos:prefLabel>
        <skos:prefLabel xml:lang="en">principal stage 1</skos:prefLabel>
        <skos:prefLabel xml:lang="fr">stade principal 1</skos:prefLabel>
    </owl:Class>
    


    <!-- http://ontology.inrae.fr/ppdo/ontology/PrincipalStage2 -->

    <owl:Class rdf:about="http://ontology.inrae.fr/ppdo/ontology/PrincipalStage2">
        <rdfs:subClassOf rdf:resource="http://ontology.inrae.fr/ppdo/ontology/PrincipalGrowthStage"/>
        <rdfs:seeAlso rdf:datatype="http://www.w3.org/2001/XMLSchema#string">http://aims.fao.org/aos/agrovoc/c_7773</rdfs:seeAlso>
        <skos:definition xml:lang="de">Bildung von Seitensprossen / Bestok­kung (Quelle BBCH Monografie)</skos:definition>
        <skos:definition xml:lang="es">Formación de brotes laterales / macollamiento (ahijamiento) (fuente BBCH monografia)</skos:definition>
        <skos:definition xml:lang="en">Formation of side shoots / tillering (source BBCH monograph)</skos:definition>
        <skos:definition xml:lang="fr">formation des pousses secondaires / tallage (source BBCH monographie)</skos:definition>
        <skos:prefLabel xml:lang="de">Makrostadium 2</skos:prefLabel>
        <skos:prefLabel xml:lang="es">estadio principal 2</skos:prefLabel>
        <skos:prefLabel xml:lang="en">principal stage 2</skos:prefLabel>
        <skos:prefLabel xml:lang="fr">stade principal 2</skos:prefLabel>
    </owl:Class>
    


    <!-- http://ontology.inrae.fr/ppdo/ontology/PrincipalStage3 -->

    <owl:Class rdf:about="http://ontology.inrae.fr/ppdo/ontology/PrincipalStage3">
        <rdfs:subClassOf rdf:resource="http://ontology.inrae.fr/ppdo/ontology/PrincipalGrowthStage"/>
        <rdfs:seeAlso rdf:datatype="http://www.w3.org/2001/XMLSchema#string">http://aims.fao.org/aos/agrovoc/c_7387</rdfs:seeAlso>
        <skos:definition xml:lang="en"> Stem elongation or rosette growth / shoot development (main shoot) (source BBCH monograph)</skos:definition>
        <skos:definition xml:lang="es">Crecimiento longitudinal del tallo o crecimiento en roseta, desarrollo de brotes (retoños)/ encañado (tallo principal) (fuente BBCH monografia)</skos:definition>
        <skos:definition xml:lang="de">Längen- bzw. Rosettenwachstum desHauptsprosses/ Triebentwicklung / Schossen (Haupt­trieb) (Quelle BBCH Monografie)</skos:definition>
        <skos:definition xml:lang="fr">élongation de la tige / formation de la rosette / développement des pousses (tige principale) (source BBCH monographie)</skos:definition>
        <skos:prefLabel xml:lang="de">Makrostadium 3</skos:prefLabel>
        <skos:prefLabel xml:lang="es">estadio principal 3</skos:prefLabel>
        <skos:prefLabel xml:lang="en">principal stage 3</skos:prefLabel>
        <skos:prefLabel xml:lang="fr">stade principal 3</skos:prefLabel>
    </owl:Class>
    


    <!-- http://ontology.inrae.fr/ppdo/ontology/PrincipalStage4 -->

    <owl:Class rdf:about="http://ontology.inrae.fr/ppdo/ontology/PrincipalStage4">
        <rdfs:subClassOf rdf:resource="http://ontology.inrae.fr/ppdo/ontology/PrincipalGrowthStage"/>
        <rdfs:seeAlso rdf:datatype="http://www.w3.org/2001/XMLSchema#string">http://aims.fao.org/aos/agrovoc/c_330641</rdfs:seeAlso>
        <skos:definition xml:lang="es">Desarrollo de las partes vegetativas cosechables de la planta o de órganos vegetativos de propagación / embuchamiento (fuente BBCH monografia)</skos:definition>
        <skos:definition xml:lang="en">Development of harvestable vegetative plant parts or vegetatively propagated organs / booting (main shoot) (source BBCH monograph)</skos:definition>
        <skos:definition xml:lang="de">Entwicklung vegetativer Pflanzenteile (Erntegut) bzw. vegetativer Vermehrungsorgane/ Ähren- bzw. Ris­penschwellen (Quelle BBCH Monografie) </skos:definition>
        <skos:definition xml:lang="fr">développement des parties végétatives de récolte ou des organes de multiplication végétative / développement des organes de reproduction sexuée, gonflement de l’épi ou de la panicule (tige principale)  (source BBCH monographie) </skos:definition>
        <skos:prefLabel xml:lang="de">Makrostadium 4</skos:prefLabel>
        <skos:prefLabel xml:lang="es">estadio principal 4</skos:prefLabel>
        <skos:prefLabel xml:lang="en">principal stage 4</skos:prefLabel>
        <skos:prefLabel xml:lang="fr">stade principal 4</skos:prefLabel>
    </owl:Class>
    


    <!-- http://ontology.inrae.fr/ppdo/ontology/PrincipalStage5 -->

    <owl:Class rdf:about="http://ontology.inrae.fr/ppdo/ontology/PrincipalStage5">
        <rdfs:subClassOf rdf:resource="http://ontology.inrae.fr/ppdo/ontology/PrincipalGrowthStage"/>
        <rdfs:seeAlso rdf:datatype="http://www.w3.org/2001/XMLSchema#string">http://aims.fao.org/aos/agrovoc/c_3510</rdfs:seeAlso>
        <skos:definition xml:lang="fr"> apparition de l’inflorescence (tige principale) / épiaison (source BBCH monographie)</skos:definition>
        <skos:definition xml:lang="es">Emergencia de la inflorescencia (tallo principal) / espigamiento (fuente BBCH monografia)</skos:definition>
        <skos:definition xml:lang="de">Erscheinen der Blütenanlage (Hauptspro ß)/ Ähren- bzw. Rispenschieben (Quelle BBCH Monografie) </skos:definition>
        <skos:definition xml:lang="en">Inflorescence emergence (main shoot) / heading (source BBCH monograph)</skos:definition>
        <skos:prefLabel xml:lang="de">Makrostadium 5</skos:prefLabel>
        <skos:prefLabel xml:lang="es">estadio principal 5</skos:prefLabel>
        <skos:prefLabel xml:lang="en">principal stage 5</skos:prefLabel>
        <skos:prefLabel xml:lang="fr">stade principal 5</skos:prefLabel>
    </owl:Class>
    


    <!-- http://ontology.inrae.fr/ppdo/ontology/PrincipalStage6 -->

    <owl:Class rdf:about="http://ontology.inrae.fr/ppdo/ontology/PrincipalStage6">
        <rdfs:subClassOf rdf:resource="http://ontology.inrae.fr/ppdo/ontology/PrincipalGrowthStage"/>
        <rdfs:seeAlso rdf:datatype="http://www.w3.org/2001/XMLSchema#string">http://aims.fao.org/aos/agrovoc/c_330768 </rdfs:seeAlso>
        <skos:definition xml:lang="de">Blüte (Hauptsproß) (Quelle BBCH Monografie)</skos:definition>
        <skos:definition xml:lang="es">Floración (tallo principal) (fuente BBCH monografia)</skos:definition>
        <skos:definition xml:lang="en">Flowering (main shoot) (source BBCH monograph)</skos:definition>
        <skos:definition xml:lang="fr">floraison (tige principale) (source BBCH monographie)</skos:definition>
        <skos:prefLabel xml:lang="de">Makrostadium 6</skos:prefLabel>
        <skos:prefLabel xml:lang="es">estadio principal 6</skos:prefLabel>
        <skos:prefLabel xml:lang="en">principal stage 6</skos:prefLabel>
        <skos:prefLabel xml:lang="fr">stade principal 6</skos:prefLabel>
    </owl:Class>
    


    <!-- http://ontology.inrae.fr/ppdo/ontology/PrincipalStage7 -->

    <owl:Class rdf:about="http://ontology.inrae.fr/ppdo/ontology/PrincipalStage7">
        <rdfs:subClassOf rdf:resource="http://ontology.inrae.fr/ppdo/ontology/PrincipalGrowthStage"/>
        <rdfs:seeAlso rdf:datatype="http://www.w3.org/2001/XMLSchema#string">http://aims.fao.org/aos/agrovoc/c_15971</rdfs:seeAlso>
        <skos:definition xml:lang="es">Desarrollo del fruto (fuente BBCH monografia)</skos:definition>
        <skos:definition xml:lang="en">Development of fruit (source BBCH monograph)</skos:definition>
        <skos:definition xml:lang="de">Fruchtentwicklung (Quelle BBCH Monografie)</skos:definition>
        <skos:definition xml:lang="fr">développement des fruits (source BBCH monographie)</skos:definition>
        <skos:prefLabel xml:lang="de">Makrostadium 7</skos:prefLabel>
        <skos:prefLabel xml:lang="es">estadio principal 7</skos:prefLabel>
        <skos:prefLabel xml:lang="en">principal stage 7</skos:prefLabel>
        <skos:prefLabel xml:lang="fr">stade principal 7</skos:prefLabel>
    </owl:Class>
    


    <!-- http://ontology.inrae.fr/ppdo/ontology/PrincipalStage8 -->

    <owl:Class rdf:about="http://ontology.inrae.fr/ppdo/ontology/PrincipalStage8">
        <rdfs:subClassOf rdf:resource="http://ontology.inrae.fr/ppdo/ontology/PrincipalGrowthStage"/>
        <rdfs:seeAlso rdf:datatype="http://www.w3.org/2001/XMLSchema#string">http://aims.fao.org/aos/agrovoc/c_330756</rdfs:seeAlso>
        <skos:definition xml:lang="es">Coloración o maduración de frutos y semillas (fuente BBCH monografia)</skos:definition>
        <skos:definition xml:lang="de">Frucht- und Samenreife (Quelle BBCH Monografie)</skos:definition>
        <skos:definition xml:lang="en">Ripening or maturity of fruit and seed (source BBCH monograph)</skos:definition>
        <skos:definition xml:lang="fr">maturation des fruits ou graines (source BBCH monographie)</skos:definition>
        <skos:prefLabel xml:lang="de">Makrostadium 8</skos:prefLabel>
        <skos:prefLabel xml:lang="es">estadio principal 8</skos:prefLabel>
        <skos:prefLabel xml:lang="en">principal stage 8</skos:prefLabel>
        <skos:prefLabel xml:lang="fr">stade principal 8</skos:prefLabel>
    </owl:Class>
    


    <!-- http://ontology.inrae.fr/ppdo/ontology/PrincipalStage9 -->

    <owl:Class rdf:about="http://ontology.inrae.fr/ppdo/ontology/PrincipalStage9">
        <rdfs:subClassOf rdf:resource="http://ontology.inrae.fr/ppdo/ontology/PrincipalGrowthStage"/>
        <rdfs:seeAlso rdf:datatype="http://www.w3.org/2001/XMLSchema#string">http://aims.fao.org/aos/agrovoc/c_14200</rdfs:seeAlso>
        <skos:definition xml:lang="de">Absterben bzw. Eintreten der Vegeta­tionsruhe (Quelle BBCH Monografie)</skos:definition>
        <skos:definition xml:lang="en">Senescence, beginning of dormancy (source BBCH monograph)</skos:definition>
        <skos:definition xml:lang="es">Senescencia, comienzo de la dormancia (fuente BBCH monografia)</skos:definition>
        <skos:definition xml:lang="fr">sénescence et mort ou début de la période de dormance (source BBCH monographie)</skos:definition>
        <skos:prefLabel xml:lang="de">Makrostadium 9</skos:prefLabel>
        <skos:prefLabel xml:lang="es">estadio principal 9</skos:prefLabel>
        <skos:prefLabel xml:lang="en">principal stage 9</skos:prefLabel>
        <skos:prefLabel xml:lang="fr">stade principal 9</skos:prefLabel>
    </owl:Class>
    


    <!-- http://ontology.inrae.fr/ppdo/ontology/SecondaryGrowthStage -->

    <owl:Class rdf:about="http://ontology.inrae.fr/ppdo/ontology/SecondaryGrowthStage">
        <owl:equivalentClass>
            <owl:Class>
                <owl:intersectionOf rdf:parseType="Collection">
                    <rdf:Description rdf:about="http://ontology.inrae.fr/ppdo/ontology/GrowthStage"/>
                    <owl:Restriction>
                        <owl:onProperty rdf:resource="http://ontology.inrae.fr/ppdo/ontology/hasRank"/>
                        <owl:hasValue rdf:resource="http://ontology.inrae.fr/ppdo/ontology/secondary"/>
                    </owl:Restriction>
                </owl:intersectionOf>
            </owl:Class>
        </owl:equivalentClass>
        <rdfs:subClassOf rdf:resource="http://ontology.inrae.fr/ppdo/ontology/GrowthStage"/>
        <skos:definition xml:lang="de">Ist eine präzise Angabe von Zeitpunkten in der Pflanzenentwicklung erforderlich, finden die Mikrostadien Verwendung. Im Gegensatz zu den Makrostadien sind sie als kurze, für die jeweilige Pflanzenart charakteristische Entwicklungsschritte definiert, die im jeweiligen Makrostadium nacheinander durchlaufen werden. Ihre Codierung erfolgt ebenfalls mit den Ziffern O bis 9. Beide Ziffern, sowohl für das Makro- als auch für das Mikrostadium, ergeben den zweistelligen Code.
Für die Mehrzahl der Pflanzenarten wird mit dem zweistelligen Code eine Skala angeboten, die eine präzise Erfassung aller phänologischen Entwicklungsstadien ermöglicht. Lediglich bei einigen Pflanzenarten (z.B. Kartoffeln, Tomaten, Gurken und Zwiebeln) kann es notwendig sein, innerhalb eines Makrostadiums eine weitere Unterteilung vorzunehmen, als es durch die Verwendung der Mikrostadien von O bis 9 möglich ist.
Für diese Fälle wird neben der zweistelligen auch eine dreistellige Skala vorgestellt. Dabei erfolgt mit dem sogenannten Mesostadium, das zwischen Makro- und Mikrostadium eingeführt wird, eine weitere Unterteilung in der Weise, daß mit den Ziffern O und 1 das Entwicklungsgeschehen am Hauptsproß und mit den Ziffern 2
bis 9 das der Seitensprosse 2. bis 9. Ordnung be_schrieben wird. So können am Hauptsproß bis zu 19 Blätter gezählt oder das Verzweigungsgeschehen beschrieben werden.
(Quelle BBCH monografie)</skos:definition>
        <skos:definition xml:lang="es">Los estadios secundarios son usados para describir con precisión fases cortas del desarrollo de plantas. En contraste a los estadios principales de crecimiento, ellos son definidos en pasos cortos de desarrollo de las respectivas especies de plantas, ocurriendo durante un determinado estadio principal de desarrollo. Ellos también son codificados usando números de 0 a 9. La combinación de los números de un estadio principal de crecimiento y el número de un estadio secundario de crecimiento conducen al código digital de 2 cifras.
El código de 2 dígitos es una escala que ofrece la posibilidad de precisar y definir todos los estadios fenológicos para la mayoría de las especies de plantas. Sólo en algunos casos (ej. pepino, cebolla, papa, tomate) se necesita una subdivisión más detallada junto a un estadio principal de crecimiento que vaya más allá de las posibilidades de uso de los estadios secundarios del 0 al 9. 
Para estos casos se presenta una escala de 3 dígitos al lado de la escala de 2 dígitos. Esto implica la inclusión de los también llamados mesoestadios entre los estadios principales y secundarios, que da origen a una subdivisión ampliada. Los mesoestadios 0 y 1 describen el tallo principal y los mesoestadios 2 al 9 describen los brotes laterales de 2o a 9o orden. En este caso se pueden contar hasta 19 hojas del tallo principal y además existe la posibilidad de describir las ramificaciones de las plantas.
(fuente BBCH monografia)</skos:definition>
        <skos:definition xml:lang="fr">On utilise les stades de développement secondaires pour déterminer un moment exact du développement. Par rapport aux stades principaux, les stades secondaires définissent des étapes limitées dans le temps. Ils sont donnés par des valeurs de 0 à 9, qui se suivent à l’intérieur d’un stade principal. On obtient ainsi un code à deux chiffres composé par le stade principal et le stade secondaire.
L’échelle de codification à 2 chiffres permet pour la plupart des espèces une description précise du stade phénologique. Néanmoins il peut être nécessaire pour certaines espèces (par exemple: pomme de terre, tomate, soja, concombre et oignon) d’introduire des codes intermédiaires qui subdivisent une nouvelle fois les stades principaux. Ainsi nous obtenons à côté des codes à 2 chiffres des codes à 3 chiffres. Le stade intermédiaire s’insérant entre le stade principal et le stade secondaire. On utilise les chiffres 0 et 1 pour la description de la tige principale, les chiffres de 2 à 9 correspondent aux pousses secondaires. Ceci permet de compter sur la tige principale jusqu’à 19 feuilles ou de décrire les pousses latérales.
(source BBCH monographie)</skos:definition>
        <skos:definition xml:lang="en">Secondary stages are used if points of time or steps in the plant
development must be indicated precisely. In contrast to the principal growth stages they are defined as short developmental steps characteristic of the respective plant species, which are passed successively during the respective principal growth stage. They are also coded by using the figures 0 to 9. The combination of figures for the principal and the secondary stages, results in the two-digit code.
The two-digit code is a scale which offers the possibility of precisely defining all phenological growth stages for the majority of plant species. Only in the case of some plant species (e.g. cucumber, onion, potato, soybean, tomato) is further subdivision necessary within a principal growth stage beyond that possible using the secondary stages from 0 to 9. For these cases a three-digit scale is presented alongside the two-digit scale. This involves the inclusion of the so-called mesostage between the principal and the secondary stage, which provides a further subdivision... In this way up to 19 leaves can be counted on the main stem or the branching can be described.
(source BBCH monograph)</skos:definition>
        <skos:prefLabel xml:lang="de">mikrostadium</skos:prefLabel>
        <skos:prefLabel xml:lang="en">secondary growth stage</skos:prefLabel>
        <skos:prefLabel xml:lang="fr">stade de développement secondaire</skos:prefLabel>
    </owl:Class>
    


    <!-- http://ontology.inrae.fr/ppdo/ontology/SecondaryStage00 -->

    <owl:Class rdf:about="http://ontology.inrae.fr/ppdo/ontology/SecondaryStage00">
        <rdfs:subClassOf rdf:resource="http://ontology.inrae.fr/ppdo/ontology/TwoDigitsSecondaryGrowthStage"/>
        <skos:definition xml:lang="en">Dry seed (seed dressing takes place at stage 00), (P, V) Winter dormancy or resting period  (source BBCH monograph)</skos:definition>
        <skos:definition xml:lang="es">Semilla seca, (los tratamientos de la semilla se efectúan en el estadio 00), (P,V) Dormancia invernal o período de reposo (fuente BBCH monografia)</skos:definition>
        <skos:definition xml:lang="de">Trockener Samen (Stadium für die Saatgutbehandlung), (V) Überdauerungs- bzw. Vermehrungsorgan im Ruhestadium, (P) Winter- bzw. Vegetationsruhe (Quelle BBCH Monografie)</skos:definition>
        <skos:definition xml:lang="fr">semence sèche (le traitement des graines avant le semis intervient au stade 00), (P, V) période de dormance hivernale ou période de repos  (source BBCH monographie)</skos:definition>
        <skos:prefLabel xml:lang="de">Mikrostadium 00</skos:prefLabel>
        <skos:prefLabel xml:lang="es">estadio secondario 00</skos:prefLabel>
        <skos:prefLabel xml:lang="en">secondary growth stage 00</skos:prefLabel>
        <skos:prefLabel xml:lang="fr">stade secondaire 00</skos:prefLabel>
    </owl:Class>
    


    <!-- http://ontology.inrae.fr/ppdo/ontology/SecondaryStage01 -->

    <owl:Class rdf:about="http://ontology.inrae.fr/ppdo/ontology/SecondaryStage01">
        <rdfs:subClassOf rdf:resource="http://ontology.inrae.fr/ppdo/ontology/TwoDigitsSecondaryGrowthStage"/>
        <skos:definition xml:lang="de">Beginn der Samenquellung, (P,V) Beginn des Knospenschwellens (Quelle BBCH Monografie)</skos:definition>
        <skos:definition xml:lang="en">Beginning of seed imbibition, (P, V) Beginning of bud swelling  (source BBCH monograph)</skos:definition>
        <skos:definition xml:lang="es">Comienza la imbibición de la semilla, (P,V) Comienza la hinchazón de la yema (fuente BBCH monografia)</skos:definition>
        <skos:definition xml:lang="fr">début de l’imbibition de la graine , (P, V) début du gonflement des bourgeons  (source BBCH monographie)</skos:definition>
        <skos:prefLabel xml:lang="de">Mikrostadium 01</skos:prefLabel>
        <skos:prefLabel xml:lang="es">estadio secondario 01</skos:prefLabel>
        <skos:prefLabel xml:lang="en">secondary growth stage 01</skos:prefLabel>
        <skos:prefLabel xml:lang="fr">stade secondaire 01</skos:prefLabel>
    </owl:Class>
    


    <!-- http://ontology.inrae.fr/ppdo/ontology/SecondaryStage03 -->

    <owl:Class rdf:about="http://ontology.inrae.fr/ppdo/ontology/SecondaryStage03">
        <rdfs:subClassOf rdf:resource="http://ontology.inrae.fr/ppdo/ontology/TwoDigitsSecondaryGrowthStage"/>
        <skos:definition xml:lang="de">Ende der Samenquellung, (P,V) Ende des Knospenschwellens (Quelle BBCH Monografie)</skos:definition>
        <skos:definition xml:lang="es">Imbibición completa, (P,V) Fin del hinchamiento de la yema (fuente BBCH monografia)</skos:definition>
        <skos:definition xml:lang="en">Seed imbibition complete, (P, V) End of bud swelling  (source BBCH monograph)</skos:definition>
        <skos:definition xml:lang="fr">l’imbibition des graines est complète, (P, V) le gonflement des bourgeons est achevé (source BBCH monographie)</skos:definition>
        <skos:prefLabel xml:lang="de">Mikrostadium 03</skos:prefLabel>
        <skos:prefLabel xml:lang="es">estadio secondario 03</skos:prefLabel>
        <skos:prefLabel xml:lang="en">secondary growth stage 03</skos:prefLabel>
        <skos:prefLabel xml:lang="fr">stade secondaire 03</skos:prefLabel>
    </owl:Class>
    


    <!-- http://ontology.inrae.fr/ppdo/ontology/SecondaryStage05 -->

    <owl:Class rdf:about="http://ontology.inrae.fr/ppdo/ontology/SecondaryStage05">
        <rdfs:subClassOf rdf:resource="http://ontology.inrae.fr/ppdo/ontology/TwoDigitsSecondaryGrowthStage"/>
        <skos:definition xml:lang="de">Keimwurzel aus dem Samen ausgetreten, (P,V) Überdauerungs- bzw. Vermehrungsorgane beginnen sich zu bewurzeln (Quelle BBCH Monografie)</skos:definition>
        <skos:definition xml:lang="es">La radícula (raíz embrional) emerge de la semilla, (P,V) Los órganos de multiplicación vegetativa comienzan a emitir raíces (fuente BBCH monografia)</skos:definition>
        <skos:definition xml:lang="en">Radicle (root) emerged from seed, (P, V) Perennating organs forming roots  (source BBCH monograph)</skos:definition>
        <skos:definition xml:lang="fr">la radicule sort de la graine , (P, V) les organes pérennes (les organes végétatifs de réserve ou de multiplication) développent des racines (source BBCH monographie)</skos:definition>
        <skos:prefLabel xml:lang="de">Mikrostadium 05</skos:prefLabel>
        <skos:prefLabel xml:lang="es">estadio secondario 05</skos:prefLabel>
        <skos:prefLabel xml:lang="en">secondary growth stage 05</skos:prefLabel>
        <skos:prefLabel xml:lang="fr">stade secondaire 05</skos:prefLabel>
    </owl:Class>
    


    <!-- http://ontology.inrae.fr/ppdo/ontology/SecondaryStage06 -->

    <owl:Class rdf:about="http://ontology.inrae.fr/ppdo/ontology/SecondaryStage06">
        <rdfs:subClassOf rdf:resource="http://ontology.inrae.fr/ppdo/ontology/TwoDigitsSecondaryGrowthStage"/>
        <skos:definition xml:lang="es">Elongación de la radícula, formación de pelos radiculares y/o raíces laterales (fuente BBCH monografia)</skos:definition>
        <skos:definition xml:lang="en">Elongation of radicle, formation of root hairs and /or lateral roots  (source BBCH monograph)</skos:definition>
        <skos:definition xml:lang="de">Keimwurzel verlängert, bildet Wurzelhaare und/oder Seitenwurzeln (Quelle BBCH Monografie)</skos:definition>
        <skos:definition xml:lang="fr">élongation de la radicule, développement des poils absorbants et / ou des racines secondaires  (source BBCH monographie)</skos:definition>
        <skos:prefLabel xml:lang="de">Mikrostadium 06</skos:prefLabel>
        <skos:prefLabel xml:lang="es">estadio secondario 06</skos:prefLabel>
        <skos:prefLabel xml:lang="en">secondary growth stage 06</skos:prefLabel>
        <skos:prefLabel xml:lang="fr">stade secondaire 06</skos:prefLabel>
    </owl:Class>
    


    <!-- http://ontology.inrae.fr/ppdo/ontology/SecondaryStage07 -->

    <owl:Class rdf:about="http://ontology.inrae.fr/ppdo/ontology/SecondaryStage07">
        <rdfs:subClassOf rdf:resource="http://ontology.inrae.fr/ppdo/ontology/TwoDigitsSecondaryGrowthStage"/>
        <skos:definition xml:lang="en">(G) Coleoptile emerged from caryopsis, (D, M) Hypocotyl with cotyledons or shoot breaking through seed coat, (P, V) Beginning of sprouting or bud breaking  (source BBCH monograph)</skos:definition>
        <skos:definition xml:lang="es">(G) El coleóptilo emerge de la semilla (cariópside), (D, M) El hipocótilo con los cotiledones o la raíz salen a través del tegumento seminal, (P,V) La yema comienza a abrirse o a brotar  (fuente BBCH monografia)</skos:definition>
        <skos:definition xml:lang="de">(G) Keimscheide (Koleoptile) aus dem Samen ausgetreten, (D, M) Hypokotyl mit Keimblättern bzw. Sproß hat Samenschale durchbrochen, (P,V) Beginn des Sproß- bzw. Knospenaustriebes (Quelle BBCH Monografie)</skos:definition>
        <skos:definition xml:lang="fr">(G) le coléoptile sort de la graine, (D, M) les téguments de la graine sont percés par l’hypocotyle et ses cotylédons ou par la jeune pousse, (P, V) début du développement des pousses ou des bourgeons  (source BBCH monographie)</skos:definition>
        <skos:prefLabel xml:lang="de">Mikrostadium 07</skos:prefLabel>
        <skos:prefLabel xml:lang="es">estadio secondario 07</skos:prefLabel>
        <skos:prefLabel xml:lang="en">secondary growth stage 07</skos:prefLabel>
        <skos:prefLabel xml:lang="fr">stade secondaire 07</skos:prefLabel>
    </owl:Class>
    


    <!-- http://ontology.inrae.fr/ppdo/ontology/SecondaryStage08 -->

    <owl:Class rdf:about="http://ontology.inrae.fr/ppdo/ontology/SecondaryStage08">
        <rdfs:subClassOf rdf:resource="http://ontology.inrae.fr/ppdo/ontology/TwoDigitsSecondaryGrowthStage"/>
        <skos:definition xml:lang="es">(D) El hipocótilo con los cotiledones crecen, dirigiéndose hacia la superficie del suelo, (P,V) El brote crece, dirigiéndose hacia la superficie del suelo  (fuente BBCH monografia)</skos:definition>
        <skos:definition xml:lang="en">(D) Hypocotyl with cotyledons growing towards soil surface, (P, V) Shoot growing towards soil surface  (source BBCH monograph)</skos:definition>
        <skos:definition xml:lang="de">(D) Hypokotyl mit Keimblättern bzw. Sproß wächst zur Bodenoberfläche, (P,V) Sproß wächst zur Bodenoberfläche (Quelle BBCH Monografie)</skos:definition>
        <skos:definition xml:lang="fr">(D) hypocotyle et cotylédons se dirigent vers la surface du sol, (P, V) les jeunes pousses se dirigent vers la surface du sol (source BBCH monographie)</skos:definition>
        <skos:prefLabel xml:lang="de">Mikrostadium 08</skos:prefLabel>
        <skos:prefLabel xml:lang="es">estadio secondario 08</skos:prefLabel>
        <skos:prefLabel xml:lang="en">secondary growth stage 08</skos:prefLabel>
        <skos:prefLabel xml:lang="fr">stade secondaire 08</skos:prefLabel>
    </owl:Class>
    


    <!-- http://ontology.inrae.fr/ppdo/ontology/SecondaryStage09 -->

    <owl:Class rdf:about="http://ontology.inrae.fr/ppdo/ontology/SecondaryStage09">
        <rdfs:subClassOf rdf:resource="http://ontology.inrae.fr/ppdo/ontology/TwoDigitsSecondaryGrowthStage"/>
        <skos:definition xml:lang="de">(G) Auflaufen: Keimscheide durchbricht Bodenoberfläche, (D,M) Auflaufen: Keimblätter durchbrechen Bodenoberfläche (außer bei hypogäischer Keimung), (D,V) Auflaufen: Sproß bzw. Blatt durchbricht die Bodenoberfläche, (P) Knospen zeigen grüne Spitzen (Quelle BBCH Monografie)</skos:definition>
        <skos:definition xml:lang="en">(G) Emergence: Coleoptile breaks through soil surface, (D, M) Emergence: Cotyledons break through soil surface (except hypogeal germination), (D, V) Emergence: Shoot/leaf breaks through soil surface, (P) Bud shows green tips (source BBCH monograph)</skos:definition>
        <skos:definition xml:lang="es">(G) Emergencia: El coleóptilo sale a través de la superficie del suelo, (D,M) Emergencia: Los cotiledones salen a través de la superficie del suelo (excepto en la germinación hipogea), (D,V) Emergencia: Brotes / hojas salen a través de la superficie del suelo, (P) La yema muestra bordes verdes  (fuente BBCH monografia)</skos:definition>
        <skos:definition xml:lang="fr">(G) levée: le coléoptile perce la surface du sol, (D, M) levée: les cotylédons percent la surface du sol (exceptée pour la germination hypogée), (D, V) levée: la jeune pousse / la feuille perce la surface du sol, (P) les bourgeons présentent des pointes vertes (source BBCH monographie)</skos:definition>
        <skos:prefLabel xml:lang="de">Mikrostadium 09</skos:prefLabel>
        <skos:prefLabel xml:lang="es">estadio secondario 09</skos:prefLabel>
        <skos:prefLabel xml:lang="en">secondary growth stage 09</skos:prefLabel>
        <skos:prefLabel xml:lang="fr">stade secondaire 09</skos:prefLabel>
    </owl:Class>
    


    <!-- http://ontology.inrae.fr/ppdo/ontology/SecondaryStage10 -->

    <owl:Class rdf:about="http://ontology.inrae.fr/ppdo/ontology/SecondaryStage10">
        <rdfs:subClassOf rdf:resource="http://ontology.inrae.fr/ppdo/ontology/TwoDigitsSecondaryGrowthStage"/>
        <skos:definition xml:lang="de">(G) Erstes Laubblatt aus der Koleoptile ausgetreten, (D,M) Keimblätter voll entfaltet, (P) Erste Blätter spreizen sich ab (Quelle BBCH Monografie)</skos:definition>
        <skos:definition xml:lang="en">(G) First true leaf emerged from coleoptile, (D, M) Cotyledons completely unfolded, (P) First leaves separated (source BBCH monograph)</skos:definition>
        <skos:definition xml:lang="es">(G) La 1a hoja verdadera emerge del coleóptilo, (D,M) Cotiledones completamente desenrollados,(P) Las primeras hojas se separan del brote (fuente BBCH monografia)</skos:definition>
        <skos:definition xml:lang="fr">(G) la première feuille sort du coléoptile, (D, M) les cotylédons sont complètement développés, (P) les premières feuilles s’étalent (source BBCH monographie)</skos:definition>
        <skos:prefLabel xml:lang="de">Mikrostadium 10</skos:prefLabel>
        <skos:prefLabel xml:lang="es">estadio secondario 10</skos:prefLabel>
        <skos:prefLabel xml:lang="en">secondary stage 10</skos:prefLabel>
        <skos:prefLabel xml:lang="fr">stade secondaire 10</skos:prefLabel>
    </owl:Class>
    


    <!-- http://ontology.inrae.fr/ppdo/ontology/SecondaryStage11 -->

    <owl:Class rdf:about="http://ontology.inrae.fr/ppdo/ontology/SecondaryStage11">
        <rdfs:subClassOf rdf:resource="http://ontology.inrae.fr/ppdo/ontology/TwoDigitsSecondaryGrowthStage"/>
        <skos:definition xml:lang="de">1. Laubblatt bzw. Blattpaar oder Blattquirl entfaltet, (P) Erste Laubblätter entfaltet (Quelle BBCH Monografie)</skos:definition>
        <skos:definition xml:lang="es">Desarrollo de la 1a hoja o par de hojas verdaderas o verticilio, (P) Desarrollo de la primera hoja (fuente BBCH monografia)</skos:definition>
        <skos:definition xml:lang="en">First true leaf, leaf pair or whorl unfolded, (P) First leaves unfolded (source BBCH monograph)</skos:definition>
        <skos:definition xml:lang="fr">la première feuille, la première paire de feuilles ou le premier verticille de feuilles est complètement étalé, (P) les premières feuilles sont étalées (source BBCH monographie)</skos:definition>
        <skos:prefLabel xml:lang="de">Mikrostadium 11</skos:prefLabel>
        <skos:prefLabel xml:lang="es">estadio secondario 11</skos:prefLabel>
        <skos:prefLabel xml:lang="en">secondary stage 11</skos:prefLabel>
        <skos:prefLabel xml:lang="fr">stade secondaire 11</skos:prefLabel>
    </owl:Class>
    


    <!-- http://ontology.inrae.fr/ppdo/ontology/SecondaryStage12 -->

    <owl:Class rdf:about="http://ontology.inrae.fr/ppdo/ontology/SecondaryStage12">
        <rdfs:subClassOf rdf:resource="http://ontology.inrae.fr/ppdo/ontology/TwoDigitsSecondaryGrowthStage"/>
        <skos:definition xml:lang="en">2 true leaves, leaf pairs or whorls unfolded (source BBCH monograph)</skos:definition>
        <skos:definition xml:lang="de">2. Laubblatt bzw. Blattpaar oder Blattquirl entfaltet (Quelle BBCH Monografie)</skos:definition>
        <skos:definition xml:lang="es">Desarrollo de la segunda hoja, o par de hojas verdaderas o verticilio (fuente BBCH monografia)</skos:definition>
        <skos:definition xml:lang="fr">la deuxième feuille, la deuxième paire de feuilles ou le deuxième verticille de feuilles est complètement étalé (source BBCH monographie)</skos:definition>
        <skos:prefLabel xml:lang="de">Mikrostadium 12</skos:prefLabel>
        <skos:prefLabel xml:lang="es">estadio secondario 12</skos:prefLabel>
        <skos:prefLabel xml:lang="en">secondary stage 12</skos:prefLabel>
        <skos:prefLabel xml:lang="fr">stade secondaire 12</skos:prefLabel>
    </owl:Class>
    


    <!-- http://ontology.inrae.fr/ppdo/ontology/SecondaryStage13 -->

    <owl:Class rdf:about="http://ontology.inrae.fr/ppdo/ontology/SecondaryStage13">
        <rdfs:subClassOf rdf:resource="http://ontology.inrae.fr/ppdo/ontology/TwoDigitsSecondaryGrowthStage"/>
        <skos:definition xml:lang="en">3 true leaves, leaf pairs or whorls unfolded (source BBCH monograph)</skos:definition>
        <skos:definition xml:lang="de">3. Laubblatt bzw. Blattpaar oder Blattquirl entfaltet (Quelle BBCH Monografie)</skos:definition>
        <skos:definition xml:lang="es">Desarrollo de la tercera hoja o par de hojas verdaderas o verticilio (fuente BBCH monografia)</skos:definition>
        <skos:definition xml:lang="fr">la troisième feuille, la troisième paire de feuilles ou le troisième verticille de feuilles est complètement étalé (source BBCH monographie)</skos:definition>
        <skos:prefLabel xml:lang="de">Mikrostadium 13</skos:prefLabel>
        <skos:prefLabel xml:lang="es">estadio secondario 13</skos:prefLabel>
        <skos:prefLabel xml:lang="en">secondary stage 13</skos:prefLabel>
        <skos:prefLabel xml:lang="fr">stade secondaire 13</skos:prefLabel>
    </owl:Class>
    


    <!-- http://ontology.inrae.fr/ppdo/ontology/SecondaryStage14 -->

    <owl:Class rdf:about="http://ontology.inrae.fr/ppdo/ontology/SecondaryStage14">
        <rdfs:subClassOf rdf:resource="http://ontology.inrae.fr/ppdo/ontology/TwoDigitsSecondaryGrowthStage"/>
        <skos:definition xml:lang="en">4 true leaves, leaf pairs or whorls unfolded (source BBCH monograph)</skos:definition>
        <skos:definition xml:lang="de">4. Laubblatt bzw. Blattpaar oder Blattquirl entfaltet (Quelle BBCH Monografie)</skos:definition>
        <skos:definition xml:lang="es">Desarrollo de la cuarto hoja o par de hojas verdaderas o verticilio (fuente BBCH monografia)</skos:definition>
        <skos:definition xml:lang="fr">la quatrième feuille, la quatrième paire de feuilles ou le quatrième verticille de feuilles est complètement étalé (source BBCH monographie)</skos:definition>
        <skos:prefLabel xml:lang="de">Mikrostadium 14</skos:prefLabel>
        <skos:prefLabel xml:lang="es">estadio secondario 14</skos:prefLabel>
        <skos:prefLabel xml:lang="en">secondary stage 14</skos:prefLabel>
        <skos:prefLabel xml:lang="fr">stade secondaire 14</skos:prefLabel>
    </owl:Class>
    


    <!-- http://ontology.inrae.fr/ppdo/ontology/SecondaryStage15 -->

    <owl:Class rdf:about="http://ontology.inrae.fr/ppdo/ontology/SecondaryStage15">
        <rdfs:subClassOf rdf:resource="http://ontology.inrae.fr/ppdo/ontology/TwoDigitsSecondaryGrowthStage"/>
        <skos:definition xml:lang="en">5 true leaves, leaf pairs or whorls unfolded (source BBCH monograph)</skos:definition>
        <skos:definition xml:lang="de">5. Laubblatt bzw. Blattpaar oder Blattquirl entfaltet (Quelle BBCH Monografie)</skos:definition>
        <skos:definition xml:lang="es">Desarrollo de la quinto hoja o par de hojas verdaderas o verticilio (fuente BBCH monografia)</skos:definition>
        <skos:definition xml:lang="fr">la cinquième feuille, la cinquième paire de feuilles ou le cinquième verticille de feuilles est complètement étalé (source BBCH monographie)</skos:definition>
        <skos:prefLabel xml:lang="de">Mikrostadium 15</skos:prefLabel>
        <skos:prefLabel xml:lang="es">estadio secondario 15</skos:prefLabel>
        <skos:prefLabel xml:lang="en">secondary stage 15</skos:prefLabel>
        <skos:prefLabel xml:lang="fr">stade secondaire 15</skos:prefLabel>
    </owl:Class>
    


    <!-- http://ontology.inrae.fr/ppdo/ontology/SecondaryStage16 -->

    <owl:Class rdf:about="http://ontology.inrae.fr/ppdo/ontology/SecondaryStage16">
        <rdfs:subClassOf rdf:resource="http://ontology.inrae.fr/ppdo/ontology/TwoDigitsSecondaryGrowthStage"/>
        <skos:definition xml:lang="en">6 true leaves, leaf pairs or whorls unfolded (source BBCH monograph)</skos:definition>
        <skos:definition xml:lang="de">6. Laubblatt bzw. Blattpaar oder Blattquirl entfaltet (Quelle BBCH Monografie)</skos:definition>
        <skos:definition xml:lang="es">Desarrollo de la sexto hoja o par de hojas verdaderas o verticilio (fuente BBCH monografia)</skos:definition>
        <skos:definition xml:lang="fr">la sixième feuille, la sixième paire de feuilles ou le sixième verticille de feuilles est complètement étalé (source BBCH monographie)</skos:definition>
        <skos:prefLabel xml:lang="de">Mikrostadium 16</skos:prefLabel>
        <skos:prefLabel xml:lang="es">estadio secondario 16</skos:prefLabel>
        <skos:prefLabel xml:lang="en">secondary stage 16</skos:prefLabel>
        <skos:prefLabel xml:lang="fr">stade secondaire 16</skos:prefLabel>
    </owl:Class>
    


    <!-- http://ontology.inrae.fr/ppdo/ontology/SecondaryStage17 -->

    <owl:Class rdf:about="http://ontology.inrae.fr/ppdo/ontology/SecondaryStage17">
        <rdfs:subClassOf rdf:resource="http://ontology.inrae.fr/ppdo/ontology/TwoDigitsSecondaryGrowthStage"/>
        <skos:definition xml:lang="en">7 true leaves, leaf pairs or whorls unfolded (source BBCH monograph)</skos:definition>
        <skos:definition xml:lang="de">7. Laubblatt bzw. Blattpaar oder Blattquirl entfaltet (Quelle BBCH Monografie)</skos:definition>
        <skos:definition xml:lang="es">Desarrollo de la séptimo hoja o par de hojas verdaderas o verticilio (fuente BBCH monografia)</skos:definition>
        <skos:definition xml:lang="fr">la septième feuille, la septième paire de feuilles ou le septième verticille de feuilles est complètement étalé (source BBCH monographie)</skos:definition>
        <skos:prefLabel xml:lang="de">Mikrostadium 17</skos:prefLabel>
        <skos:prefLabel xml:lang="es">estadio secondario 17</skos:prefLabel>
        <skos:prefLabel xml:lang="en">secondary stage 17</skos:prefLabel>
        <skos:prefLabel xml:lang="fr">stade secondaire 17</skos:prefLabel>
    </owl:Class>
    


    <!-- http://ontology.inrae.fr/ppdo/ontology/SecondaryStage18 -->

    <owl:Class rdf:about="http://ontology.inrae.fr/ppdo/ontology/SecondaryStage18">
        <rdfs:subClassOf rdf:resource="http://ontology.inrae.fr/ppdo/ontology/TwoDigitsSecondaryGrowthStage"/>
        <skos:definition xml:lang="en">8 true leaves, leaf pairs or whorls unfolded (source BBCH monograph)</skos:definition>
        <skos:definition xml:lang="de">8. Laubblatt bzw. Blattpaar oder Blattquirl entfaltet (Quelle BBCH Monografie)</skos:definition>
        <skos:definition xml:lang="es">Desarrollo de la octavo hoja o par de hojas verdaderas o verticilio (fuente BBCH monografia)</skos:definition>
        <skos:definition xml:lang="fr">la huitième feuille, la huitième paire de feuilles ou le huitième verticille de feuilles est complètement étalé (source BBCH monographie)</skos:definition>
        <skos:prefLabel xml:lang="de">Mikrostadium 18</skos:prefLabel>
        <skos:prefLabel xml:lang="es">estadio secondario 18</skos:prefLabel>
        <skos:prefLabel xml:lang="en">secondary stage 18</skos:prefLabel>
        <skos:prefLabel xml:lang="fr">stade secondaire 18</skos:prefLabel>
    </owl:Class>
    


    <!-- http://ontology.inrae.fr/ppdo/ontology/SecondaryStage19 -->

    <owl:Class rdf:about="http://ontology.inrae.fr/ppdo/ontology/SecondaryStage19">
        <rdfs:subClassOf rdf:resource="http://ontology.inrae.fr/ppdo/ontology/TwoDigitsSecondaryGrowthStage"/>
        <skos:definition xml:lang="de">9 oder mehr Laubblätter bzw. Blattpaare oder Blattquirle entfaltet (Quelle BBCH Monografie)</skos:definition>
        <skos:definition xml:lang="en">9 or more true leaves, leaf pairs or whorls unfolded (source BBCH monograph)</skos:definition>
        <skos:definition xml:lang="fr">9 ou davantage de feuilles, de paires de feuilles, ou de verticilles sont étalés (source BBCH monographie)</skos:definition>
        <skos:definition xml:lang="es">Desarrollo de 9 o más hojas verdaderas o pares de hojas o verticilios (fuente BBCH monografia)</skos:definition>
        <skos:prefLabel xml:lang="de">Mikrostadium 19</skos:prefLabel>
        <skos:prefLabel xml:lang="es">estadio secondario 19</skos:prefLabel>
        <skos:prefLabel xml:lang="en">secondary stage 19</skos:prefLabel>
        <skos:prefLabel xml:lang="fr">stade secondaire 19</skos:prefLabel>
    </owl:Class>
    


    <!-- http://ontology.inrae.fr/ppdo/ontology/SecondaryStage21 -->

    <owl:Class rdf:about="http://ontology.inrae.fr/ppdo/ontology/SecondaryStage21">
        <rdfs:subClassOf rdf:resource="http://ontology.inrae.fr/ppdo/ontology/TwoDigitsSecondaryGrowthStage"/>
        <skos:definition xml:lang="de">1. Seitensproß sichtbar, (G) 1. Bestockungstrieb sichtbar (Quelle BBCH Monografie)</skos:definition>
        <skos:definition xml:lang="es">1er brote lateral visible, (G) 1er hijuelo o macolla visible (fuente BBCH monografia)</skos:definition>
        <skos:definition xml:lang="en">First side shoot visible, (G) First tiller visible (source BBCH monograph)</skos:definition>
        <skos:definition xml:lang="fr">première pousse secondaire visible, (G) premier talle visible  (source BBCH monographie)</skos:definition>
        <skos:prefLabel xml:lang="de">Mikrostadium 21</skos:prefLabel>
        <skos:prefLabel xml:lang="es">estadio secondario 21</skos:prefLabel>
        <skos:prefLabel xml:lang="en">secondary stage 21</skos:prefLabel>
        <skos:prefLabel xml:lang="fr">stade secondaire 21</skos:prefLabel>
    </owl:Class>
    


    <!-- http://ontology.inrae.fr/ppdo/ontology/SecondaryStage22 -->

    <owl:Class rdf:about="http://ontology.inrae.fr/ppdo/ontology/SecondaryStage22">
        <rdfs:subClassOf rdf:resource="http://ontology.inrae.fr/ppdo/ontology/TwoDigitsSecondaryGrowthStage"/>
        <skos:definition xml:lang="fr">2 pousses secondaires visibles, (G) 2 talles visibles  (source BBCH monographie)</skos:definition>
        <skos:definition xml:lang="en">2 side shoots visible, (G) 2 tillers visible (source BBCH monograph)</skos:definition>
        <skos:definition xml:lang="de">2. Seitensproß sichtbar, (G) 2. Bestockungstrieb sichtbar (Quelle BBCH Monografie)</skos:definition>
        <skos:definition xml:lang="es">2o brote lateral visible, (G) 2o hijuelo o macolla visible (fuente BBCH monografia)</skos:definition>
        <skos:prefLabel xml:lang="de">Mikrostadium 22</skos:prefLabel>
        <skos:prefLabel xml:lang="es">estadio secondario 22</skos:prefLabel>
        <skos:prefLabel xml:lang="en">secondary stage 22</skos:prefLabel>
        <skos:prefLabel xml:lang="fr">stade secondaire 22</skos:prefLabel>
    </owl:Class>
    


    <!-- http://ontology.inrae.fr/ppdo/ontology/SecondaryStage23 -->

    <owl:Class rdf:about="http://ontology.inrae.fr/ppdo/ontology/SecondaryStage23">
        <rdfs:subClassOf rdf:resource="http://ontology.inrae.fr/ppdo/ontology/TwoDigitsSecondaryGrowthStage"/>
        <skos:definition xml:lang="fr">3 pousses secondaires visibles, (G) 3 talles visibles  (source BBCH monographie)</skos:definition>
        <skos:definition xml:lang="en">3 side shoots visible, (G) 3 tillers visible  (source BBCH monograph)</skos:definition>
        <skos:definition xml:lang="de">3. Seitensproß sichtbar, (G) 3. Bestockungstrieb sichtbar (Quelle BBCH Monografie)</skos:definition>
        <skos:definition xml:lang="es">3er brote lateral visible, (G) 3er hijuelo o macolla visible (fuente BBCH monografia)</skos:definition>
        <skos:prefLabel xml:lang="de">Mikrostadium 23</skos:prefLabel>
        <skos:prefLabel xml:lang="es">estadio secondario 23</skos:prefLabel>
        <skos:prefLabel xml:lang="en">secondary stage 23</skos:prefLabel>
        <skos:prefLabel xml:lang="fr">stade secondaire 23</skos:prefLabel>
    </owl:Class>
    


    <!-- http://ontology.inrae.fr/ppdo/ontology/SecondaryStage24 -->

    <owl:Class rdf:about="http://ontology.inrae.fr/ppdo/ontology/SecondaryStage24">
        <rdfs:subClassOf rdf:resource="http://ontology.inrae.fr/ppdo/ontology/TwoDigitsSecondaryGrowthStage"/>
        <skos:definition xml:lang="fr">4 pousses secondaires visibles, (G) 4 talles visibles  (source BBCH monographie)</skos:definition>
        <skos:definition xml:lang="en">4 side shoots visible, (G) 4 tillers visible  (source BBCH monograph)</skos:definition>
        <skos:definition xml:lang="de">4. Seitensproß sichtbar, (G) 4. Bestockungstrieb sichtbar (Quelle BBCH Monografie)</skos:definition>
        <skos:definition xml:lang="es">4o brote lateral visible, (G) 4o hijuelo o macolla visible (fuente BBCH monografia)</skos:definition>
        <skos:prefLabel xml:lang="de">Mikrostadium 24</skos:prefLabel>
        <skos:prefLabel xml:lang="es">estadio secondario 24</skos:prefLabel>
        <skos:prefLabel xml:lang="en">secondary stage 24</skos:prefLabel>
        <skos:prefLabel xml:lang="fr">stade secondaire 24</skos:prefLabel>
    </owl:Class>
    


    <!-- http://ontology.inrae.fr/ppdo/ontology/SecondaryStage25 -->

    <owl:Class rdf:about="http://ontology.inrae.fr/ppdo/ontology/SecondaryStage25">
        <rdfs:subClassOf rdf:resource="http://ontology.inrae.fr/ppdo/ontology/TwoDigitsSecondaryGrowthStage"/>
        <skos:definition xml:lang="fr">5 pousses secondaires visibles, (G) 5 talles visibles  (source BBCH monographie)</skos:definition>
        <skos:definition xml:lang="en">5 side shoots visible, (G) 5 tillers visible  (source BBCH monograph)</skos:definition>
        <skos:definition xml:lang="de">5. Seitensproß sichtbar, (G) 5. Bestockungstrieb sichtbar (Quelle BBCH Monografie)</skos:definition>
        <skos:definition xml:lang="es">5o brote lateral visible, (G) 5o hijuelo o macolla visible (fuente BBCH monografia)</skos:definition>
        <skos:prefLabel xml:lang="de">Mikrostadium 25</skos:prefLabel>
        <skos:prefLabel xml:lang="es">estadio secondario 25</skos:prefLabel>
        <skos:prefLabel xml:lang="en">secondary stage 25</skos:prefLabel>
        <skos:prefLabel xml:lang="fr">stade secondaire 25</skos:prefLabel>
    </owl:Class>
    


    <!-- http://ontology.inrae.fr/ppdo/ontology/SecondaryStage26 -->

    <owl:Class rdf:about="http://ontology.inrae.fr/ppdo/ontology/SecondaryStage26">
        <rdfs:subClassOf rdf:resource="http://ontology.inrae.fr/ppdo/ontology/TwoDigitsSecondaryGrowthStage"/>
        <skos:definition xml:lang="fr">6 pousses secondaires visibles, (G) 6 talles visibles  (source BBCH monographie)</skos:definition>
        <skos:definition xml:lang="en">6 side shoots visible, (G) 6 tillers visible  (source BBCH monograph)</skos:definition>
        <skos:definition xml:lang="de">6. Seitensproß sichtbar, (G) 6. Bestockungstrieb sichtbar (Quelle BBCH Monografie)</skos:definition>
        <skos:definition xml:lang="es">6o brote lateral visible, (G) 6o hijuelo o macolla visible (fuente BBCH monografia)</skos:definition>
        <skos:prefLabel xml:lang="de">Mikrostadium 26</skos:prefLabel>
        <skos:prefLabel xml:lang="es">estadio secondario 26</skos:prefLabel>
        <skos:prefLabel xml:lang="en">secondary stage 26</skos:prefLabel>
        <skos:prefLabel xml:lang="fr">stade secondaire 26</skos:prefLabel>
    </owl:Class>
    


    <!-- http://ontology.inrae.fr/ppdo/ontology/SecondaryStage27 -->

    <owl:Class rdf:about="http://ontology.inrae.fr/ppdo/ontology/SecondaryStage27">
        <rdfs:subClassOf rdf:resource="http://ontology.inrae.fr/ppdo/ontology/TwoDigitsSecondaryGrowthStage"/>
        <skos:definition xml:lang="fr">7 pousses secondaires visibles, (G) 7 talles visibles  (source BBCH monographie)</skos:definition>
        <skos:definition xml:lang="en">7 side shoots visible, (G) 7 tillers visible  (source BBCH monograph)</skos:definition>
        <skos:definition xml:lang="de">7. Seitensproß sichtbar, (G) 7. Bestockungstrieb sichtbar (Quelle BBCH Monografie)</skos:definition>
        <skos:definition xml:lang="es">7o brote lateral visible, (G) 7o hijuelo o macolla visible (fuente BBCH monografia)</skos:definition>
        <skos:prefLabel xml:lang="de">Mikrostadium 27</skos:prefLabel>
        <skos:prefLabel xml:lang="es">estadio secondario 27</skos:prefLabel>
        <skos:prefLabel xml:lang="en">secondary stage 27</skos:prefLabel>
        <skos:prefLabel xml:lang="fr">stade secondaire 27</skos:prefLabel>
    </owl:Class>
    


    <!-- http://ontology.inrae.fr/ppdo/ontology/SecondaryStage28 -->

    <owl:Class rdf:about="http://ontology.inrae.fr/ppdo/ontology/SecondaryStage28">
        <rdfs:subClassOf rdf:resource="http://ontology.inrae.fr/ppdo/ontology/TwoDigitsSecondaryGrowthStage"/>
        <skos:definition xml:lang="fr">8 pousses secondaires visibles, (G) 8 talles visibles  (source BBCH monographie)</skos:definition>
        <skos:definition xml:lang="en">8 side shoots visible, (G) 8 tillers visible  (source BBCH monograph)</skos:definition>
        <skos:definition xml:lang="de">8. Seitensproß sichtbar, (G) 8. Bestockungstrieb sichtbar (Quelle BBCH Monografie)</skos:definition>
        <skos:definition xml:lang="es">8o brote lateral visible, (G) 8o hijuelo o macolla visible (fuente BBCH monografia)</skos:definition>
        <skos:prefLabel xml:lang="de">Mikrostadium 28</skos:prefLabel>
        <skos:prefLabel xml:lang="es">estadio secondario 28</skos:prefLabel>
        <skos:prefLabel xml:lang="en">secondary stage 28</skos:prefLabel>
        <skos:prefLabel xml:lang="fr">stade secondaire 28</skos:prefLabel>
    </owl:Class>
    


    <!-- http://ontology.inrae.fr/ppdo/ontology/SecondaryStage29 -->

    <owl:Class rdf:about="http://ontology.inrae.fr/ppdo/ontology/SecondaryStage29">
        <rdfs:subClassOf rdf:resource="http://ontology.inrae.fr/ppdo/ontology/TwoDigitsSecondaryGrowthStage"/>
        <skos:definition xml:lang="es">9 o más brotes laterales visibles, (G) 9 o más hijuelos o macollas visibles (fuente BBCH monografia)</skos:definition>
        <skos:definition xml:lang="de">9 oder mehr Seitensprosse sichtbar, (G) 9 oder mehr Bestockungstriebe sichtbar (Quelle BBCH Monografie)</skos:definition>
        <skos:definition xml:lang="en">9 or more side shoots visible, (G) 9 or more tillers visible (source BBCH monograph)</skos:definition>
        <skos:definition xml:lang="fr">9 ou davantage de pousses secondaires visibles, (G) 9 ou davantage de talles visibles  (source BBCH monographie)</skos:definition>
        <skos:prefLabel xml:lang="de">Mikrostadium 29</skos:prefLabel>
        <skos:prefLabel xml:lang="es">estadio secondario 29</skos:prefLabel>
        <skos:prefLabel xml:lang="en">secondary stage 29</skos:prefLabel>
        <skos:prefLabel xml:lang="fr">stade secondaire 29</skos:prefLabel>
    </owl:Class>
    


    <!-- http://ontology.inrae.fr/ppdo/ontology/SecondaryStage31 -->

    <owl:Class rdf:about="http://ontology.inrae.fr/ppdo/ontology/SecondaryStage31">
        <rdfs:subClassOf rdf:resource="http://ontology.inrae.fr/ppdo/ontology/TwoDigitsSecondaryGrowthStage"/>
        <skos:definition xml:lang="de">10% des arttypischen max. Längen- bzw. Rosettenwachstums erreicht, (G) 1-Knoten-Stadium (Quelle BBCH Monografie)</skos:definition>
        <skos:definition xml:lang="es">El tallo o la roseta han alcanzado el 10% de su longitud o grosor final, (G) 1 nudo detectable (fuente BBCH monografia)</skos:definition>
        <skos:definition xml:lang="en">Stem (rosette) 10% of final length (diameter), (G) 1 node detectable  (source BBCH monograph )</skos:definition>
        <skos:definition xml:lang="fr">la tige (la rosette) atteint 10% de sa longueur définitive (de son diamètre définitif), (G) 1 nœud est discernable sur la tige principale  (source BBCH monographie)</skos:definition>
        <skos:prefLabel xml:lang="de">Mikrostadium 31</skos:prefLabel>
        <skos:prefLabel xml:lang="es">estadio secondario 31</skos:prefLabel>
        <skos:prefLabel xml:lang="en">secondary stage 31</skos:prefLabel>
        <skos:prefLabel xml:lang="fr">stade secondaire 31</skos:prefLabel>
    </owl:Class>
    


    <!-- http://ontology.inrae.fr/ppdo/ontology/SecondaryStage32 -->

    <owl:Class rdf:about="http://ontology.inrae.fr/ppdo/ontology/SecondaryStage32">
        <rdfs:subClassOf rdf:resource="http://ontology.inrae.fr/ppdo/ontology/TwoDigitsSecondaryGrowthStage"/>
        <skos:definition xml:lang="de">20% des arttypischen max. Längen- bzw. Rosettenwachstums erreicht, (G) 2-Knoten-Stadium (Quelle BBCH Monografie)</skos:definition>
        <skos:definition xml:lang="es">El tallo o la roseta han alcanzado el 20% de la longitud o el grosor final, (G) 2 nudos detectables (fuente BBCH monografia)</skos:definition>
        <skos:definition xml:lang="en">Stem (rosette) 20% of final length (diameter), (G) 2 nodes detectable  (source BBCH monograph)</skos:definition>
        <skos:definition xml:lang="fr">la tige (la rosette) atteint 20% de sa longueur définitive (de son diamètre définitif), (G) 2 nœuds sont discernables  (source BBCH monographie)</skos:definition>
        <skos:prefLabel xml:lang="de">Mikrostadium 32</skos:prefLabel>
        <skos:prefLabel xml:lang="es">estadio secondario 32</skos:prefLabel>
        <skos:prefLabel xml:lang="en">secondary stage 32</skos:prefLabel>
        <skos:prefLabel xml:lang="fr">stade secondaire 32</skos:prefLabel>
    </owl:Class>
    


    <!-- http://ontology.inrae.fr/ppdo/ontology/SecondaryStage33 -->

    <owl:Class rdf:about="http://ontology.inrae.fr/ppdo/ontology/SecondaryStage33">
        <rdfs:subClassOf rdf:resource="http://ontology.inrae.fr/ppdo/ontology/TwoDigitsSecondaryGrowthStage"/>
        <skos:definition xml:lang="de">30% des arttypischen max. Längen- bzw. Rosettenwachstums erreicht, (G) 3-Knoten-Stadium (Quelle BBCH Monografie)</skos:definition>
        <skos:definition xml:lang="es">El tallo o la roseta han alcanzado el 30% de la longitud o el grosor final, (G) 3 nudos detectables (fuente BBCH monografia)</skos:definition>
        <skos:definition xml:lang="en">Stem (rosette) 30% of final length (diameter), (G) 3 nodes detectable  (source BBCH monograph)</skos:definition>
        <skos:definition xml:lang="fr">la tige (la rosette) atteint 30% de sa longueur définitive (de son diamètre définitif), (G) 3 nœuds sont discernables  (source BBCH monographie)</skos:definition>
        <skos:prefLabel xml:lang="de">Mikrostadium 33</skos:prefLabel>
        <skos:prefLabel xml:lang="es">estadio secondario 33</skos:prefLabel>
        <skos:prefLabel xml:lang="en">secondary stage 33</skos:prefLabel>
        <skos:prefLabel xml:lang="fr">stade secondaire 33</skos:prefLabel>
    </owl:Class>
    


    <!-- http://ontology.inrae.fr/ppdo/ontology/SecondaryStage34 -->

    <owl:Class rdf:about="http://ontology.inrae.fr/ppdo/ontology/SecondaryStage34">
        <rdfs:subClassOf rdf:resource="http://ontology.inrae.fr/ppdo/ontology/TwoDigitsSecondaryGrowthStage"/>
        <skos:definition xml:lang="de">40% des arttypischen max. Längen- bzw. Rosettenwachstums erreicht, (G) 4-Knoten-Stadium (Quelle BBCH Monografie)</skos:definition>
        <skos:definition xml:lang="es">El tallo o la roseta han alcanzado el 40% de la longitud o el grosor final, (G) 4 nudos detectables (fuente BBCH monografia)</skos:definition>
        <skos:definition xml:lang="en">Stem (rosette) 40% of final length (diameter), (G) 4 nodes detectable  (source BBCH monograph)</skos:definition>
        <skos:definition xml:lang="fr">la tige (la rosette) atteint 40% de sa longueur définitive (de son diamètre définitif), (G) 4 nœuds sont discernables  (source BBCH monographie)</skos:definition>
        <skos:prefLabel xml:lang="de">Mikrostadium 34</skos:prefLabel>
        <skos:prefLabel xml:lang="es">estadio secondario 34</skos:prefLabel>
        <skos:prefLabel xml:lang="en">secondary stage 34</skos:prefLabel>
        <skos:prefLabel xml:lang="fr">stade secondaire 34</skos:prefLabel>
    </owl:Class>
    


    <!-- http://ontology.inrae.fr/ppdo/ontology/SecondaryStage35 -->

    <owl:Class rdf:about="http://ontology.inrae.fr/ppdo/ontology/SecondaryStage35">
        <rdfs:subClassOf rdf:resource="http://ontology.inrae.fr/ppdo/ontology/TwoDigitsSecondaryGrowthStage"/>
        <skos:definition xml:lang="de">50% des arttypischen max. Längen- bzw. Rosettenwachstums erreicht, (G) 5-Knoten-Stadium (Quelle BBCH Monografie)</skos:definition>
        <skos:definition xml:lang="es">El tallo o la roseta han alcanzado el 50% de la longitud o el grosor final, (G) 5 nudos detectables (fuente BBCH monografia)</skos:definition>
        <skos:definition xml:lang="en">Stem (rosette) 50% of final length (diameter), (G) 5 nodes detectable  (source BBCH monograph)</skos:definition>
        <skos:definition xml:lang="fr">la tige (la rosette) atteint 50% de sa longueur définitive (de son diamètre définitif), (G) 5 nœuds sont discernables  (source BBCH monographie)</skos:definition>
        <skos:prefLabel xml:lang="de">Mikrostadium 35</skos:prefLabel>
        <skos:prefLabel xml:lang="es">estadio secondario 35</skos:prefLabel>
        <skos:prefLabel xml:lang="en">secondary stage 35</skos:prefLabel>
        <skos:prefLabel xml:lang="fr">stade secondaire 35</skos:prefLabel>
    </owl:Class>
    


    <!-- http://ontology.inrae.fr/ppdo/ontology/SecondaryStage36 -->

    <owl:Class rdf:about="http://ontology.inrae.fr/ppdo/ontology/SecondaryStage36">
        <rdfs:subClassOf rdf:resource="http://ontology.inrae.fr/ppdo/ontology/TwoDigitsSecondaryGrowthStage"/>
        <skos:definition xml:lang="de">60% des arttypischen max. Längen- bzw. Rosettenwachstums erreicht, (G) 6-Knoten-Stadium (Quelle BBCH Monografie)</skos:definition>
        <skos:definition xml:lang="es">El tallo o la roseta han alcanzado el 60% de la longitud o el grosor final, (G) 6 nudos detectables (fuente BBCH monografia)</skos:definition>
        <skos:definition xml:lang="en">Stem (rosette) 60% of final length (diameter), (G) 6 nodes detectable  (source BBCH monograph )</skos:definition>
        <skos:definition xml:lang="fr">la tige (la rosette) atteint 60% de sa longueur définitive (de son diamètre définitif), (G) 6 nœuds sont discernables  (source BBCH monographie)</skos:definition>
        <skos:prefLabel xml:lang="de">Mikrostadium 36</skos:prefLabel>
        <skos:prefLabel xml:lang="es">estadio secondario 36</skos:prefLabel>
        <skos:prefLabel xml:lang="en">secondary stage 36</skos:prefLabel>
        <skos:prefLabel xml:lang="fr">stade secondaire 36</skos:prefLabel>
    </owl:Class>
    


    <!-- http://ontology.inrae.fr/ppdo/ontology/SecondaryStage37 -->

    <owl:Class rdf:about="http://ontology.inrae.fr/ppdo/ontology/SecondaryStage37">
        <rdfs:subClassOf rdf:resource="http://ontology.inrae.fr/ppdo/ontology/TwoDigitsSecondaryGrowthStage"/>
        <skos:definition xml:lang="de">70% des arttypischen max. Längen- bzw. Rosettenwachstums erreicht, (G) 7-Knoten-Stadium (Quelle BBCH Monografie)</skos:definition>
        <skos:definition xml:lang="es">El tallo o la roseta han alcanzado el 70% de la longitud o el grosor final, (G) 7 nudos detectables (fuente BBCH monografia)</skos:definition>
        <skos:definition xml:lang="en">Stem (rosette) 70% of final length (diameter), (G) 7 nodes detectable  (source BBCH monograph)</skos:definition>
        <skos:definition xml:lang="fr">la tige (la rosette) atteint 70% de sa longueur définitive (de son diamètre définitif), (G) 7 nœuds sont discernables  (source BBCH monographie)</skos:definition>
        <skos:prefLabel xml:lang="de">Mikrostadium 37</skos:prefLabel>
        <skos:prefLabel xml:lang="es">estadio secondario 37</skos:prefLabel>
        <skos:prefLabel xml:lang="en">secondary stage 37</skos:prefLabel>
        <skos:prefLabel xml:lang="fr">stade secondaire 37</skos:prefLabel>
    </owl:Class>
    


    <!-- http://ontology.inrae.fr/ppdo/ontology/SecondaryStage38 -->

    <owl:Class rdf:about="http://ontology.inrae.fr/ppdo/ontology/SecondaryStage38">
        <rdfs:subClassOf rdf:resource="http://ontology.inrae.fr/ppdo/ontology/TwoDigitsSecondaryGrowthStage"/>
        <skos:definition xml:lang="de">80% des arttypischen max. Längen- bzw. Rosettenwachstums erreicht, (G) 8-Knoten-Stadium (Quelle BBCH Monografie)</skos:definition>
        <skos:definition xml:lang="es">El tallo o la roseta han alcanzado el 80% de la longitud o el grosor final, (G) 8 nudos detectables (fuente BBCH monografia)</skos:definition>
        <skos:definition xml:lang="en">Stem (rosette) 80% of final length (diameter), (G) 8 nodes detectable  (source BBCH monograph)</skos:definition>
        <skos:definition xml:lang="fr">la tige (la rosette) atteint 80% de sa longueur définitive (de son diamètre définitif), (G) 8 nœuds sont discernables  (source BBCH monographie)</skos:definition>
        <skos:prefLabel xml:lang="de">Mikrostadium 38</skos:prefLabel>
        <skos:prefLabel xml:lang="es">estadio secondario 38</skos:prefLabel>
        <skos:prefLabel xml:lang="en">secondary stage 38</skos:prefLabel>
        <skos:prefLabel xml:lang="fr">stade secondaire 38</skos:prefLabel>
    </owl:Class>
    


    <!-- http://ontology.inrae.fr/ppdo/ontology/SecondaryStage39 -->

    <owl:Class rdf:about="http://ontology.inrae.fr/ppdo/ontology/SecondaryStage39">
        <rdfs:subClassOf rdf:resource="http://ontology.inrae.fr/ppdo/ontology/TwoDigitsSecondaryGrowthStage"/>
        <skos:definition xml:lang="es">El tallo o la roseta han alcanzado el máximo de la longitud o el grosor final, (G) 9 o más nudos detectables (fuente BBCH monografia)</skos:definition>
        <skos:definition xml:lang="de">Maximale Länge bzw. Durchmesser erreicht, (G) 9 oder mehr Knoten (Quelle BBCH Monografie)</skos:definition>
        <skos:definition xml:lang="en">Maximum stem length or rosette diameter reached, (G) 9 or more nodes detectable  (source BBCH monograph)</skos:definition>
        <skos:definition xml:lang="fr">la tige (la rosette) atteint sa longueur maximale (son diamètre maximal), (G) 9 ou davantage de nœuds sont discernables  (source BBCH monographie)</skos:definition>
        <skos:prefLabel xml:lang="de">Mikrostadium 39</skos:prefLabel>
        <skos:prefLabel xml:lang="es">estadio secondario 39</skos:prefLabel>
        <skos:prefLabel xml:lang="en">secondary stage 39</skos:prefLabel>
        <skos:prefLabel xml:lang="fr">stade secondaire 39</skos:prefLabel>
    </owl:Class>
    


    <!-- http://ontology.inrae.fr/ppdo/ontology/SecondaryStage40 -->

    <owl:Class rdf:about="http://ontology.inrae.fr/ppdo/ontology/SecondaryStage40">
        <rdfs:subClassOf rdf:resource="http://ontology.inrae.fr/ppdo/ontology/TwoDigitsSecondaryGrowthStage"/>
        <skos:definition xml:lang="de">Beginn der Entwicklung vegetativen Erntegutes bzw. vegetativer Vermehrungsorgane (Quelle BBCH Monografie)</skos:definition>
        <skos:definition xml:lang="en">Harvestable vegetative plant parts or vegetatively propagated organs begin to develop  (source BBCH monograph)</skos:definition>
        <skos:definition xml:lang="es">Se inicia el desarrollo de las partes vegetativas cosechables de la planta o de los órganos de propagación vegetativa (fuente BBCH monografia)</skos:definition>
        <skos:definition xml:lang="fr">début du développement des organes végétatifs de récolte ou de multiplication  (source BBCH monographie)</skos:definition>
        <skos:prefLabel xml:lang="de">Mikrostadium 40</skos:prefLabel>
        <skos:prefLabel xml:lang="es">estadio secondario 40</skos:prefLabel>
        <skos:prefLabel xml:lang="en">secondary stage 40</skos:prefLabel>
        <skos:prefLabel xml:lang="fr">stade secondaire 40</skos:prefLabel>
    </owl:Class>
    


    <!-- http://ontology.inrae.fr/ppdo/ontology/SecondaryStage41 -->

    <owl:Class rdf:about="http://ontology.inrae.fr/ppdo/ontology/SecondaryStage41">
        <rdfs:subClassOf rdf:resource="http://ontology.inrae.fr/ppdo/ontology/TwoDigitsSecondaryGrowthStage"/>
        <skos:definition xml:lang="de">(G) Blattscheide des Fahnenblattes verlängert sich (Quelle BBCH Monografie)</skos:definition>
        <skos:definition xml:lang="en">(G) Flag leaf sheath extending  (source BBCH monograph)</skos:definition>
        <skos:definition xml:lang="es">(G) La vaina de la hoja bandera se alarga (fuente BBCH monografia)</skos:definition>
        <skos:definition xml:lang="fr">(G) élongation de la gaine foliaire de la dernière feuille  (source BBCH monographie)</skos:definition>
        <skos:prefLabel xml:lang="de">Mikrostadium 41</skos:prefLabel>
        <skos:prefLabel xml:lang="es">estadio secondario 41</skos:prefLabel>
        <skos:prefLabel xml:lang="en">secondary stage 42</skos:prefLabel>
        <skos:prefLabel xml:lang="fr">stade secondaire 41</skos:prefLabel>
    </owl:Class>
    


    <!-- http://ontology.inrae.fr/ppdo/ontology/SecondaryStage43 -->

    <owl:Class rdf:about="http://ontology.inrae.fr/ppdo/ontology/SecondaryStage43">
        <rdfs:subClassOf rdf:resource="http://ontology.inrae.fr/ppdo/ontology/TwoDigitsSecondaryGrowthStage"/>
        <skos:definition xml:lang="en">Harvestable vegetative plant parts or vegetatively propagated organs have reached 30% of final size, (G) Flag leaf sheath just visibly swollen (mid-boot) (source BBCH monograph)</skos:definition>
        <skos:definition xml:lang="es">Las partes vegetativas cosechables o los órganos de propagación vegetativa han alcanzado el 30% de su tamaño definitivo, (G) La vaina de la hoja bandera empieza a hincharse (embucharse) (fuente BBCH monografia)</skos:definition>
        <skos:definition xml:lang="de">Vegetatives Erntegut bzw. vegetative Vermehrungsorgane haben 30% der endgültigen Größe erreicht, (G) Blattscheide des Fahnenblattes beginnt anzuschwellen (Quelle BBCH Monografie)</skos:definition>
        <skos:definition xml:lang="fr">les organes végétatifs de récolte ou de multiplication atteignent 30% de leur taille finale, (G) début du gonflement de la gaine de la dernière feuille  (source BBCH monographie)</skos:definition>
        <skos:prefLabel xml:lang="de">Mikrostadium 43</skos:prefLabel>
        <skos:prefLabel xml:lang="es">estadio secondario 43</skos:prefLabel>
        <skos:prefLabel xml:lang="en">secondary stage 43</skos:prefLabel>
        <skos:prefLabel xml:lang="fr">stade secondaire 43</skos:prefLabel>
    </owl:Class>
    


    <!-- http://ontology.inrae.fr/ppdo/ontology/SecondaryStage45 -->

    <owl:Class rdf:about="http://ontology.inrae.fr/ppdo/ontology/SecondaryStage45">
        <rdfs:subClassOf rdf:resource="http://ontology.inrae.fr/ppdo/ontology/TwoDigitsSecondaryGrowthStage"/>
        <skos:definition xml:lang="en">Harvestable vegetative plant parts or vegetatively propagated organs have reached 50% of final size, (G) Flag leaf sheath swollen (late-boot)  (source BBCH monograph)</skos:definition>
        <skos:definition xml:lang="es">Las partes vegetativas cosechables o los órganos de propagación vegetativa han alcanzado el 50% de su tamaño definitivo, (G) La vaina de la hoja bandera está hinchada (embuchada) (fuente BBCH monografia)</skos:definition>
        <skos:definition xml:lang="de">Vegetatives Erntegut bzw. vegetative Vermehrungsorgane haben 50% der endgültigen Größe erreicht, (G) Blattscheide des Fahnenblattes geschwollen (Quelle BBCH Monografie)</skos:definition>
        <skos:definition xml:lang="fr">les organes végétatifs de récolte ou de multiplication atteignent 50% de leur taille finale, (G) gonflement maximal de la gaine de la dernière feuille  (source BBCH monographie)</skos:definition>
        <skos:prefLabel xml:lang="de">Mikrostadium 45</skos:prefLabel>
        <skos:prefLabel xml:lang="es">estadio secondario 45</skos:prefLabel>
        <skos:prefLabel xml:lang="en">secondary stage 45</skos:prefLabel>
        <skos:prefLabel xml:lang="fr">stade secondaire 45</skos:prefLabel>
    </owl:Class>
    


    <!-- http://ontology.inrae.fr/ppdo/ontology/SecondaryStage47 -->

    <owl:Class rdf:about="http://ontology.inrae.fr/ppdo/ontology/SecondaryStage47">
        <rdfs:subClassOf rdf:resource="http://ontology.inrae.fr/ppdo/ontology/TwoDigitsSecondaryGrowthStage"/>
        <skos:definition xml:lang="en">Harvestable vegetative plant parts or vegetatively propagated organs have reached 70% of final size, (G) Flag leaf sheath opening  (source BBCH monograph)</skos:definition>
        <skos:definition xml:lang="es">Las partes vegetativas cosechables o los órganos de propagación vegetativa han alcanzado el 70% de su tamaño definitivo, (G) Apertura de la vaina de la hoja bandera (fuente BBCH monografia)</skos:definition>
        <skos:definition xml:lang="de">Vegetatives Erntegut bzw. vegetative Vermehrungsorgane haben 70% der endgültigen Größe erreicht, (G) Blattscheide des Fahnenblattes öffnet sich (Quelle BBCH Monografie)</skos:definition>
        <skos:definition xml:lang="fr">les organes végétatifs de récolte ou de multiplication atteignent 70% de leur taille finale, (G) ouverture de la gaine de la dernière feuille  (source BBCH monographie)</skos:definition>
        <skos:prefLabel xml:lang="de">Mikrostadium 47</skos:prefLabel>
        <skos:prefLabel xml:lang="es">estadio secondario 47</skos:prefLabel>
        <skos:prefLabel xml:lang="en">secondary stage 47</skos:prefLabel>
        <skos:prefLabel xml:lang="fr">stade secondaire 47</skos:prefLabel>
    </owl:Class>
    


    <!-- http://ontology.inrae.fr/ppdo/ontology/SecondaryStage49 -->

    <owl:Class rdf:about="http://ontology.inrae.fr/ppdo/ontology/SecondaryStage49">
        <rdfs:subClassOf rdf:resource="http://ontology.inrae.fr/ppdo/ontology/TwoDigitsSecondaryGrowthStage"/>
        <skos:definition xml:lang="en">Harvestable vegetative plant parts or vegetatively propagated organs have reached final size, (G) First awns visible  (source BBCH monograph)</skos:definition>
        <skos:definition xml:lang="es">Las partes vegetativas cosechables o los órganos de propagación vegetativa están en su momento de maduración, (G) Las aristas (barbas) se hacen visibles (fuente BBCH monografia)</skos:definition>
        <skos:definition xml:lang="de">Vegetatives Erntegut bzw. vegetative Vermehrungsorgane haben endgültige Größe erreicht, (G) Grannen sichtbar (Quelle BBCH Monografie)</skos:definition>
        <skos:definition xml:lang="fr">les organes végétatifs de récolte ou de multiplication atteignent leur taille finale, (G) premières arêtes (barbes) visibles (pour les espèces aristées)  (source BBCH monographie)</skos:definition>
        <skos:prefLabel xml:lang="de">Mikrostadium 49</skos:prefLabel>
        <skos:prefLabel xml:lang="es">estadio secondario 49</skos:prefLabel>
        <skos:prefLabel xml:lang="en">secondary stage 49</skos:prefLabel>
        <skos:prefLabel xml:lang="fr">stade secondaire 49</skos:prefLabel>
    </owl:Class>
    


    <!-- http://ontology.inrae.fr/ppdo/ontology/SecondaryStage51 -->

    <owl:Class rdf:about="http://ontology.inrae.fr/ppdo/ontology/SecondaryStage51">
        <rdfs:subClassOf rdf:resource="http://ontology.inrae.fr/ppdo/ontology/TwoDigitsSecondaryGrowthStage"/>
        <skos:definition xml:lang="de">Blütenanlagen bzw. -knospen sichtbar, (G) Beginn des Ähren- bzw. Rispenschiebens (Quelle BBCH Monografie)</skos:definition>
        <skos:definition xml:lang="en">Inflorescence or flower buds visible, (G) Beginning of heading (source BBCH monograph)</skos:definition>
        <skos:definition xml:lang="fr">inflorescence ou boutons floraux visibles, (G) début de l’épiaison (source BBCH monographie)</skos:definition>
        <skos:definition xml:lang="es">Órganos florales o botones florales visibles, (G) Se inicia la salida de las espigas o panículas (fuente BBCH monografia)</skos:definition>
        <skos:prefLabel xml:lang="de">Mikrostadium 51</skos:prefLabel>
        <skos:prefLabel xml:lang="es">estadio secondario 51</skos:prefLabel>
        <skos:prefLabel xml:lang="en">secondary stage 51</skos:prefLabel>
        <skos:prefLabel xml:lang="fr">stade secondaire 51</skos:prefLabel>
    </owl:Class>
    


    <!-- http://ontology.inrae.fr/ppdo/ontology/SecondaryStage53 -->

    <owl:Class rdf:about="http://ontology.inrae.fr/ppdo/ontology/SecondaryStage53">
        <rdfs:subClassOf rdf:resource="http://ontology.inrae.fr/ppdo/ontology/TwoDigitsSecondaryGrowthStage"/>
        <skos:definition xml:lang="de">(Weinrebe) „Gescheine&quot; (Infloreszenzen) deutlich sichtbar (Quelle BBCH Monografie)</skos:definition>
        <skos:definition xml:lang="en">(grapevigne) Inflorescence clearly visible (source  BBCH monograph)</skos:definition>
        <skos:definition xml:lang="es">(vid) Inflorescencias, claramente visibless (fuente BBCH monografia)</skos:definition>
        <skos:definition xml:lang="fr">(vigne) les grappes (inflorescences) sont nettement visibles (source BBCH monographie)</skos:definition>
        <skos:prefLabel xml:lang="de">Mikrostadium 53</skos:prefLabel>
        <skos:prefLabel xml:lang="es">estadio secondario 53</skos:prefLabel>
        <skos:prefLabel xml:lang="en">secondary stage 53</skos:prefLabel>
        <skos:prefLabel xml:lang="fr">stade secondaire 53</skos:prefLabel>
    </owl:Class>
    


    <!-- http://ontology.inrae.fr/ppdo/ontology/SecondaryStage55 -->

    <owl:Class rdf:about="http://ontology.inrae.fr/ppdo/ontology/SecondaryStage55">
        <rdfs:subClassOf rdf:resource="http://ontology.inrae.fr/ppdo/ontology/TwoDigitsSecondaryGrowthStage"/>
        <skos:definition xml:lang="de">Erste Einzelblüten sichtbar (geschlossen), (G) Mitte des Ähren- bzw. Rispenschiebens (Quelle BBCH Monografie)</skos:definition>
        <skos:definition xml:lang="en">First individual flowers visible (still closed), (G) Half of inflorescence emerged (middle of heading) (source BBCH monograph)</skos:definition>
        <skos:definition xml:lang="es">Los primeros capullos y botónes (flósculos) individuales visibles (sin abrirse), (G) Mitad de la salida de las espigas o panículas (fuente BBCH monografia)</skos:definition>
        <skos:definition xml:lang="fr">les premières fleurs sont visibles (non épanouies), (G) la moitié de l’inflorescence est sortie (mi-épiaison) (source BBCH monographie)</skos:definition>
        <skos:prefLabel xml:lang="de">Mikrostadium 55</skos:prefLabel>
        <skos:prefLabel xml:lang="es">estadio secondario 55</skos:prefLabel>
        <skos:prefLabel xml:lang="en">secondary stage 55</skos:prefLabel>
        <skos:prefLabel xml:lang="fr">stade secondaire 55</skos:prefLabel>
    </owl:Class>
    


    <!-- http://ontology.inrae.fr/ppdo/ontology/SecondaryStage57 -->

    <owl:Class rdf:about="http://ontology.inrae.fr/ppdo/ontology/SecondaryStage57">
        <rdfs:subClassOf rdf:resource="http://ontology.inrae.fr/ppdo/ontology/TwoDigitsSecondaryGrowthStage"/>
        <skos:definition xml:lang="de">(Weinrebe) „Gescheine&quot; (Infloreszenzen) sind voll entwickelt; die Einzelblüten spreizen sich (Quelle BBCH Monografie)</skos:definition>
        <skos:definition xml:lang="en">(grapevigne) Inflorescences fully developed; flowers separating (source BBCH monograph)</skos:definition>
        <skos:definition xml:lang="es">(vid) Inflorescencias, desarrolladas completamente; flores separándose (fuente BBCH monografia)</skos:definition>
        <skos:definition xml:lang="fr">(vigne) les grappes sont bien développées, les fleurs se séparent (source BBCH monographie)</skos:definition>
        <skos:prefLabel xml:lang="de">Mikrostadium 57</skos:prefLabel>
        <skos:prefLabel xml:lang="es">estadio secondario 57</skos:prefLabel>
        <skos:prefLabel xml:lang="en">secondary stage 57</skos:prefLabel>
        <skos:prefLabel xml:lang="fr">stade secondaire 57</skos:prefLabel>
    </owl:Class>
    


    <!-- http://ontology.inrae.fr/ppdo/ontology/SecondaryStage59 -->

    <owl:Class rdf:about="http://ontology.inrae.fr/ppdo/ontology/SecondaryStage59">
        <rdfs:subClassOf rdf:resource="http://ontology.inrae.fr/ppdo/ontology/TwoDigitsSecondaryGrowthStage"/>
        <skos:definition xml:lang="de">Erste Blütenblätter sichtbar, Blüten noch geschlossen, (G) Ende des Ähren- bzw. Rispenschiebens (Quelle BBCH Monografie)</skos:definition>
        <skos:definition xml:lang="en">First flower petals visible (in petalled forms), (G) Inflorescence fully emerged (end of heading) (source BBCH monograph)</skos:definition>
        <skos:definition xml:lang="es">Primeros pétalos (hojas florales) visibles, (G) Fin de la salida de las espigas o panículas (fuente BBCH monografia)</skos:definition>
        <skos:definition xml:lang="fr">les premiers pétales floraux sont visibles, la fleur est encore fermée, (G) l’inflorescence est complètement sortie (fin de l’épiaison) (source BBCH monographie)</skos:definition>
        <skos:prefLabel xml:lang="de">Mikrostadium 59</skos:prefLabel>
        <skos:prefLabel xml:lang="es">estadio secondario 59</skos:prefLabel>
        <skos:prefLabel xml:lang="en">secondary stage 59</skos:prefLabel>
        <skos:prefLabel xml:lang="fr">stade secondaire 59</skos:prefLabel>
    </owl:Class>
    


    <!-- http://ontology.inrae.fr/ppdo/ontology/SecondaryStage60 -->

    <owl:Class rdf:about="http://ontology.inrae.fr/ppdo/ontology/SecondaryStage60">
        <rdfs:subClassOf rdf:resource="http://ontology.inrae.fr/ppdo/ontology/TwoDigitsSecondaryGrowthStage"/>
        <skos:definition xml:lang="en">First flowers open (sporadically) (source BBCH monograph)</skos:definition>
        <skos:definition xml:lang="es">Primeras flores, abiertas (fuente BBCH monografia)</skos:definition>
        <skos:definition xml:lang="de">Vereinzelt erste Blüten offen (Quelle BBCH Monografie)</skos:definition>
        <skos:definition xml:lang="fr">les premières fleurs sont ouvertes (source BBCH monographie)</skos:definition>
        <skos:prefLabel xml:lang="de">Mikrostadium 60</skos:prefLabel>
        <skos:prefLabel xml:lang="es">estadio secondario 60</skos:prefLabel>
        <skos:prefLabel xml:lang="en">secondary stage 60</skos:prefLabel>
        <skos:prefLabel xml:lang="fr">stade secondaire 60</skos:prefLabel>
    </owl:Class>
    


    <!-- http://ontology.inrae.fr/ppdo/ontology/SecondaryStage61 -->

    <owl:Class rdf:about="http://ontology.inrae.fr/ppdo/ontology/SecondaryStage61">
        <rdfs:subClassOf rdf:resource="http://ontology.inrae.fr/ppdo/ontology/TwoDigitsSecondaryGrowthStage"/>
        <skos:definition xml:lang="de">Beginn der Blüte: 10% der Blüten offen (Quelle BBCH Monografie)</skos:definition>
        <skos:definition xml:lang="en">Beginning of flowering: 10% of flowers open (source BBCH monograph)</skos:definition>
        <skos:definition xml:lang="es">Comienzo de la floración: 10% de flores abiertas o 10% de plantas en floración (fuente BBCH monografia)</skos:definition>
        <skos:definition xml:lang="fr">début de la floraison: 10% des fleurs sont ouvertes (source BBCH monographie)</skos:definition>
        <skos:prefLabel xml:lang="de">Mikrostadium 61</skos:prefLabel>
        <skos:prefLabel xml:lang="es">estadio secondario 61</skos:prefLabel>
        <skos:prefLabel xml:lang="en">secondary stage 61</skos:prefLabel>
        <skos:prefLabel xml:lang="fr">stade secondaire 61</skos:prefLabel>
    </owl:Class>
    


    <!-- http://ontology.inrae.fr/ppdo/ontology/SecondaryStage62 -->

    <owl:Class rdf:about="http://ontology.inrae.fr/ppdo/ontology/SecondaryStage62">
        <rdfs:subClassOf rdf:resource="http://ontology.inrae.fr/ppdo/ontology/TwoDigitsSecondaryGrowthStage"/>
        <skos:definition xml:lang="de">20 % der Blüten offen (Quelle BBCH Monografie)</skos:definition>
        <skos:definition xml:lang="es">20% de flores abiertas o 20% de plantas en floración (fuente BBCH monografia)</skos:definition>
        <skos:definition xml:lang="fr">20% des fleurs sont ouvertes (source BBCH monographie)</skos:definition>
        <skos:definition xml:lang="en">20% of flowers open (source BBCH monograph)</skos:definition>
        <skos:prefLabel xml:lang="de">Mikrostadium 62</skos:prefLabel>
        <skos:prefLabel xml:lang="es">estadio secondario 62</skos:prefLabel>
        <skos:prefLabel xml:lang="en">secondary stage 62</skos:prefLabel>
        <skos:prefLabel xml:lang="fr">stade secondaire 62</skos:prefLabel>
    </owl:Class>
    


    <!-- http://ontology.inrae.fr/ppdo/ontology/SecondaryStage63 -->

    <owl:Class rdf:about="http://ontology.inrae.fr/ppdo/ontology/SecondaryStage63">
        <rdfs:subClassOf rdf:resource="http://ontology.inrae.fr/ppdo/ontology/TwoDigitsSecondaryGrowthStage"/>
        <skos:definition xml:lang="es">30% de flores abiertas o 30% de plantas en floración (fuente BBCH monografia)</skos:definition>
        <skos:definition xml:lang="de">30% der Blüten offen (Quelle BBCH Monografie)</skos:definition>
        <skos:definition xml:lang="fr">30% des fleurs sont ouvertes (source BBCH monographie)</skos:definition>
        <skos:definition xml:lang="en">30% of flowers open (source BBCH monograph)</skos:definition>
        <skos:prefLabel xml:lang="de">Mikrostadium 63</skos:prefLabel>
        <skos:prefLabel xml:lang="es">estadio secondario 63</skos:prefLabel>
        <skos:prefLabel xml:lang="en">secondary stage 63</skos:prefLabel>
        <skos:prefLabel xml:lang="fr">stade secondaire 63</skos:prefLabel>
    </owl:Class>
    


    <!-- http://ontology.inrae.fr/ppdo/ontology/SecondaryStage64 -->

    <owl:Class rdf:about="http://ontology.inrae.fr/ppdo/ontology/SecondaryStage64">
        <rdfs:subClassOf rdf:resource="http://ontology.inrae.fr/ppdo/ontology/TwoDigitsSecondaryGrowthStage"/>
        <skos:definition xml:lang="de">40 % der Blüten offen (Quelle BBCH Monografie)</skos:definition>
        <skos:definition xml:lang="es">40% de flores abiertas o 40% de plantas en floración (fuente BBCH monografia)</skos:definition>
        <skos:definition xml:lang="fr">40% des fleurs sont ouvertes (source BBCH monographie)</skos:definition>
        <skos:definition xml:lang="en">40% of flowers open (source BBCH monograph)</skos:definition>
        <skos:prefLabel xml:lang="de">Mikrostadium 64</skos:prefLabel>
        <skos:prefLabel xml:lang="es">estadio secondario 64</skos:prefLabel>
        <skos:prefLabel xml:lang="en">secondary stage 64</skos:prefLabel>
        <skos:prefLabel xml:lang="fr">stade secondaire 64</skos:prefLabel>
    </owl:Class>
    


    <!-- http://ontology.inrae.fr/ppdo/ontology/SecondaryStage65 -->

    <owl:Class rdf:about="http://ontology.inrae.fr/ppdo/ontology/SecondaryStage65">
        <rdfs:subClassOf rdf:resource="http://ontology.inrae.fr/ppdo/ontology/TwoDigitsSecondaryGrowthStage"/>
        <skos:definition xml:lang="en">Full flowering: 50% of flowers open, first petals may be fallen (source BBCH monograph)</skos:definition>
        <skos:definition xml:lang="es">Plena floración: 50% de las flores abiertas o 50% de las plantas en floración; los primeros pétalos caen o se secan (fuente BBCH monografia)</skos:definition>
        <skos:definition xml:lang="de">Vollblüte: 50% der Blüten offen, erste Blütenblätter können fallen oder vertrocknen (Quelle BBCH Monografie)</skos:definition>
        <skos:definition xml:lang="fr">pleine floraison: 50% des fleurs sont ouvertes, les premiers pétales tombent ou sèchent (source BBCH monographie)</skos:definition>
        <skos:prefLabel xml:lang="de">Mikrostadium 65</skos:prefLabel>
        <skos:prefLabel xml:lang="es">estadio secondario 65</skos:prefLabel>
        <skos:prefLabel xml:lang="en">secondary stage 65</skos:prefLabel>
        <skos:prefLabel xml:lang="fr">stade secondaire 65</skos:prefLabel>
    </owl:Class>
    


    <!-- http://ontology.inrae.fr/ppdo/ontology/SecondaryStage66 -->

    <owl:Class rdf:about="http://ontology.inrae.fr/ppdo/ontology/SecondaryStage66">
        <rdfs:subClassOf rdf:resource="http://ontology.inrae.fr/ppdo/ontology/TwoDigitsSecondaryGrowthStage"/>
        <skos:definition xml:lang="de">(Weinrebe) 60 % der Blütenkäppchen abgeworfen (Quelle BBCH Monografie)</skos:definition>
        <skos:definition xml:lang="en">(grapevigne) 60% of flowerhoods fallen (source BBCH monograph)</skos:definition>
        <skos:definition xml:lang="es">(vid) Alrededor de 60 % de capuchones caídos (fuente BBCH monografia)</skos:definition>
        <skos:definition xml:lang="fr">(vigne) 60% des capuchons floraux sont tombés (source BBCH monographie)</skos:definition>
        <skos:prefLabel xml:lang="de">Mikrostadium 66</skos:prefLabel>
        <skos:prefLabel xml:lang="es">estadio secondario 66</skos:prefLabel>
        <skos:prefLabel xml:lang="en">secondary stage 66</skos:prefLabel>
        <skos:prefLabel xml:lang="fr">stade secondaire 66</skos:prefLabel>
    </owl:Class>
    


    <!-- http://ontology.inrae.fr/ppdo/ontology/SecondaryStage67 -->

    <owl:Class rdf:about="http://ontology.inrae.fr/ppdo/ontology/SecondaryStage67">
        <rdfs:subClassOf rdf:resource="http://ontology.inrae.fr/ppdo/ontology/TwoDigitsSecondaryGrowthStage"/>
        <skos:definition xml:lang="de">Abgehende Blüte: Mehrzahl der Blütenblätter abgefallen oder vertrocknet (Quelle BBCH Monografie)</skos:definition>
        <skos:definition xml:lang="es">Floración llegando a su final: mayoría de los pétalos caídos o secos (fuente BBCH monografia)</skos:definition>
        <skos:definition xml:lang="en">Flowering finishing: majority of petals fallen or dry (source BBCH monograph)</skos:definition>
        <skos:definition xml:lang="fr">la floraison s’achève, la plupart des pétales sont tombés ou desséchés (source BBCH monographie)</skos:definition>
        <skos:prefLabel xml:lang="de">Mikrostadium 67</skos:prefLabel>
        <skos:prefLabel xml:lang="es">estadio secondario 67</skos:prefLabel>
        <skos:prefLabel xml:lang="en">secondary stage 67</skos:prefLabel>
        <skos:prefLabel xml:lang="fr">stade secondaire 67</skos:prefLabel>
    </owl:Class>
    


    <!-- http://ontology.inrae.fr/ppdo/ontology/SecondaryStage68 -->

    <owl:Class rdf:about="http://ontology.inrae.fr/ppdo/ontology/SecondaryStage68">
        <rdfs:subClassOf rdf:resource="http://ontology.inrae.fr/ppdo/ontology/TwoDigitsSecondaryGrowthStage"/>
        <skos:definition xml:lang="de">(Weinrebe) 80 % der Blütenkäppchen abgeworfen (Quelle BBCH Monografie)</skos:definition>
        <skos:definition xml:lang="en">(grapevigne) 80% of flowerhoods fallen (source BBCH monograph)</skos:definition>
        <skos:definition xml:lang="es">(vid) Alrededor de 80 % de capuchones caídos (fuente BBCH monografia)</skos:definition>
        <skos:definition xml:lang="fr">(vigne) la floraison s’achève: 80% des capuchons floraux sont tombés (source BBCH monographie)</skos:definition>
        <skos:prefLabel xml:lang="de">Mikrostadium 68</skos:prefLabel>
        <skos:prefLabel xml:lang="es">estadio secondario 68</skos:prefLabel>
        <skos:prefLabel xml:lang="en">secondary stage 68</skos:prefLabel>
        <skos:prefLabel xml:lang="fr">stade secondaire 68</skos:prefLabel>
    </owl:Class>
    


    <!-- http://ontology.inrae.fr/ppdo/ontology/SecondaryStage69 -->

    <owl:Class rdf:about="http://ontology.inrae.fr/ppdo/ontology/SecondaryStage69">
        <rdfs:subClassOf rdf:resource="http://ontology.inrae.fr/ppdo/ontology/TwoDigitsSecondaryGrowthStage"/>
        <skos:definition xml:lang="en">End of flowering: fruit set visible (source BBCH monograph)</skos:definition>
        <skos:definition xml:lang="de">Ende der Blüte: Fruchtansatz sichtbar (Quelle BBCH Monografie)</skos:definition>
        <skos:definition xml:lang="es">Fin de la floración: Cuajado del fruto visible (fuente BBCH monografia)</skos:definition>
        <skos:definition xml:lang="fr">fin de la floraison, le début de la formation du fruit est visible (source BBCH monographie)</skos:definition>
        <skos:prefLabel xml:lang="de">Mikrostadium 69</skos:prefLabel>
        <skos:prefLabel xml:lang="es">estadio secondario 69</skos:prefLabel>
        <skos:prefLabel xml:lang="en">secondary stage 69</skos:prefLabel>
        <skos:prefLabel xml:lang="fr">stade secondaire 69</skos:prefLabel>
    </owl:Class>
    


    <!-- http://ontology.inrae.fr/ppdo/ontology/SecondaryStage71 -->

    <owl:Class rdf:about="http://ontology.inrae.fr/ppdo/ontology/SecondaryStage71">
        <rdfs:subClassOf rdf:resource="http://ontology.inrae.fr/ppdo/ontology/TwoDigitsSecondaryGrowthStage"/>
        <skos:definition xml:lang="de">10% der Früchte erreichen art-/sortenspezifische Größe bzw. 10% der normalen Fruchtgröße erreicht, (G) Wasserreife, Korninhalt wäßrig (Quelle BBCH Monografie)</skos:definition>
        <skos:definition xml:lang="fr">10% des fruits ont atteint leur taille maximale ou les fruits atteignent 10% de leur taille finale, (G) stade aqueux du caryopse  (source BBCH monographie)</skos:definition>
        <skos:definition xml:lang="en">10% of fruits have reached final size or fruit has reached 10% of final size (G) Caryopsis watery ripe  (source BBCH monograph)</skos:definition>
        <skos:definition xml:lang="es">El 10% de los frutos alcanzan el tamaño especifico de su especie / variedad o bien el 10% del tamaño final, (G) Grano acuoso (fuente BBCH monografia)</skos:definition>
        <skos:prefLabel xml:lang="de">Mikrostadium 71</skos:prefLabel>
        <skos:prefLabel xml:lang="es">estadio secondario 71</skos:prefLabel>
        <skos:prefLabel xml:lang="en">secondary stage 71</skos:prefLabel>
        <skos:prefLabel xml:lang="fr">stade secondaire 71</skos:prefLabel>
    </owl:Class>
    


    <!-- http://ontology.inrae.fr/ppdo/ontology/SecondaryStage72 -->

    <owl:Class rdf:about="http://ontology.inrae.fr/ppdo/ontology/SecondaryStage72">
        <rdfs:subClassOf rdf:resource="http://ontology.inrae.fr/ppdo/ontology/TwoDigitsSecondaryGrowthStage"/>
        <skos:definition xml:lang="de">20 % der Früchte erreichen art-/sortenspezifische Größe bzw. 20 % der normalen Fruchtgröße erreicht (Quelle BBCH Monografie)</skos:definition>
        <skos:definition xml:lang="fr">20% des fruits ont atteint leur taille maximale ou les fruits atteignent 20% de leur taille finale  (source BBCH monographie)</skos:definition>
        <skos:definition xml:lang="en">20% of fruits have reached final size or fruit has reached 20% of final size  (source BBCH monograph)</skos:definition>
        <skos:definition xml:lang="es">El 20% de los frutos alcanzan el tamaño específico de su especie / variedad o bien el 20% del tamaño final (fuente BBCH monografia)</skos:definition>
        <skos:prefLabel xml:lang="de">Mikrostadium 72</skos:prefLabel>
        <skos:prefLabel xml:lang="es">estadio secondario 72</skos:prefLabel>
        <skos:prefLabel xml:lang="en">secondary stage 72</skos:prefLabel>
        <skos:prefLabel xml:lang="fr">stade secondaire 72</skos:prefLabel>
    </owl:Class>
    


    <!-- http://ontology.inrae.fr/ppdo/ontology/SecondaryStage73 -->

    <owl:Class rdf:about="http://ontology.inrae.fr/ppdo/ontology/SecondaryStage73">
        <rdfs:subClassOf rdf:resource="http://ontology.inrae.fr/ppdo/ontology/TwoDigitsSecondaryGrowthStage"/>
        <skos:definition xml:lang="de">30% der Früchte erreichen art-/sortenspezifische Größe bzw. 30% der normalen Fruchtgröße erreicht, (G) Frühe Milchreife (Quelle BBCH Monografie)</skos:definition>
        <skos:definition xml:lang="fr">30% des fruits ont atteint leur taille maximale ou les fruit atteignent 30% de leur taille finale, (G) début du stade laiteux du caryopse  (source BBCH monographie)</skos:definition>
        <skos:definition xml:lang="en">30% of fruits have reached final size or fruit has reached 30% of final size (G) Early milk  (source BBCH monograph)</skos:definition>
        <skos:definition xml:lang="es">El 30% de los frutos alcanzan el tamaño especifico de su especie / variedad o bien el 30% del tamaño final, (G) Lechoso temprano (fuente BBCH monografia)</skos:definition>
        <skos:prefLabel xml:lang="de">Mikrostadium 73</skos:prefLabel>
        <skos:prefLabel xml:lang="es">estadio secondario 73</skos:prefLabel>
        <skos:prefLabel xml:lang="en">secondary stage 73</skos:prefLabel>
        <skos:prefLabel xml:lang="fr">stade secondaire 73</skos:prefLabel>
    </owl:Class>
    


    <!-- http://ontology.inrae.fr/ppdo/ontology/SecondaryStage74 -->

    <owl:Class rdf:about="http://ontology.inrae.fr/ppdo/ontology/SecondaryStage74">
        <rdfs:subClassOf rdf:resource="http://ontology.inrae.fr/ppdo/ontology/TwoDigitsSecondaryGrowthStage"/>
        <skos:definition xml:lang="de">40 % der Früchte erreichen art-/sortenspezifische Größe bzw. 20 % der normalen Fruchtgröße erreicht (Quelle BBCH Monografie)</skos:definition>
        <skos:definition xml:lang="fr">40% des fruits ont atteint leur taille maximale ou les fruits atteignent 40% de leur taille finale  (source BBCH monographie)</skos:definition>
        <skos:definition xml:lang="en">40% of fruits have reached final size or fruit has reached 40% of final size  (source BBCH monograph)</skos:definition>
        <skos:definition xml:lang="es">El 40% de los frutos alcanzan el tamaño especifico de su especie / variedad o bien el 40% del tamaño final (fuente BBCH monografia)</skos:definition>
        <skos:prefLabel xml:lang="de">Mikrostadium 74</skos:prefLabel>
        <skos:prefLabel xml:lang="es">estadio secondario 74</skos:prefLabel>
        <skos:prefLabel xml:lang="en">secondary stage 74</skos:prefLabel>
        <skos:prefLabel xml:lang="fr">stade secondaire 74</skos:prefLabel>
    </owl:Class>
    


    <!-- http://ontology.inrae.fr/ppdo/ontology/SecondaryStage75 -->

    <owl:Class rdf:about="http://ontology.inrae.fr/ppdo/ontology/SecondaryStage75">
        <rdfs:subClassOf rdf:resource="http://ontology.inrae.fr/ppdo/ontology/TwoDigitsSecondaryGrowthStage"/>
        <skos:definition xml:lang="de">50% der Früchte erreichen art-/sortenspezifische Größe bzw. 50% der normalen Fruchtgröße erreicht, (G) Milchreife, Korninhalt milchig (Quelle BBCH Monografie)</skos:definition>
        <skos:definition xml:lang="fr">50% des fruits ont atteint leur taille maximale ou les fruits atteignent 50% de leur taille finale, (G) stade laiteux du caryopse  (source BBCH monographie)</skos:definition>
        <skos:definition xml:lang="en">50% of fruits have reached final size or fruit has reached 50% of final size (G) Milky ripe, medium milk  (source BBCH monograph)</skos:definition>
        <skos:definition xml:lang="es">El 50% de los frutos alcanzan el tamaño especifico de su especie / variedad o bien el 50% del tamaño final, (G) Grano lechoso (fuente BBCH monografia)</skos:definition>
        <skos:prefLabel xml:lang="de">Mikrostadium 75</skos:prefLabel>
        <skos:prefLabel xml:lang="es">estadio secondario 75</skos:prefLabel>
        <skos:prefLabel xml:lang="en">secondary stage 75</skos:prefLabel>
        <skos:prefLabel xml:lang="fr">stade secondaire 75</skos:prefLabel>
    </owl:Class>
    


    <!-- http://ontology.inrae.fr/ppdo/ontology/SecondaryStage76 -->

    <owl:Class rdf:about="http://ontology.inrae.fr/ppdo/ontology/SecondaryStage76">
        <rdfs:subClassOf rdf:resource="http://ontology.inrae.fr/ppdo/ontology/TwoDigitsSecondaryGrowthStage"/>
        <skos:definition xml:lang="de">60 % der Früchte erreichen art-/sortenspezifische Größe bzw. 20 % der normalen Fruchtgröße erreicht (Quelle BBCH Monografie)</skos:definition>
        <skos:definition xml:lang="fr">60% des fruits ont atteint leur taille maximale ou les fruits atteignent 60% de leur taille finale  (source BBCH monographie)</skos:definition>
        <skos:definition xml:lang="en">60% of fruits have reached final size or fruit has reached 60% of final size  (source BBCH monograph)</skos:definition>
        <skos:definition xml:lang="es">El 60% de los frutos alcanzan el tamaño especifico de su especie / variedad o bien el 60% del tamaño final (fuente BBCH monografia)</skos:definition>
        <skos:prefLabel xml:lang="de">Mikrostadium 76</skos:prefLabel>
        <skos:prefLabel xml:lang="es">estadio secondario 76</skos:prefLabel>
        <skos:prefLabel xml:lang="en">secondary stage 76</skos:prefLabel>
        <skos:prefLabel xml:lang="fr">stade secondaire 76</skos:prefLabel>
    </owl:Class>
    


    <!-- http://ontology.inrae.fr/ppdo/ontology/SecondaryStage77 -->

    <owl:Class rdf:about="http://ontology.inrae.fr/ppdo/ontology/SecondaryStage77">
        <rdfs:subClassOf rdf:resource="http://ontology.inrae.fr/ppdo/ontology/TwoDigitsSecondaryGrowthStage"/>
        <skos:definition xml:lang="de">70% der Früchte erreichen art-/sortenspezifische Größe bzw. 70% der normalen Fruchtgröße erreicht, (G) Späte Milchreife (Quelle BBCH Monografie)</skos:definition>
        <skos:definition xml:lang="fr">70% des fruits ont atteint leur taille maximale ou les fruit atteignent 70% de leur taille finale, (G) fin du stade laiteux du caryopse  (source BBCH monographie)</skos:definition>
        <skos:definition xml:lang="en">70% of fruits have reached final size or fruit has reached 70% of final size (G) Late milk (source BBCH monograph)</skos:definition>
        <skos:definition xml:lang="es">El 70% de los frutos alcanzan el tamaño especifico de su especie / variedad o bien el 70% del tamaño final, (G) Lechoso tardío (fuente BBCH monografia)</skos:definition>
        <skos:prefLabel xml:lang="de">Mikrostadium 77</skos:prefLabel>
        <skos:prefLabel xml:lang="es">estadio secondario 77</skos:prefLabel>
        <skos:prefLabel xml:lang="en">secondary stage 77</skos:prefLabel>
        <skos:prefLabel xml:lang="fr">stade secondaire 77</skos:prefLabel>
    </owl:Class>
    


    <!-- http://ontology.inrae.fr/ppdo/ontology/SecondaryStage78 -->

    <owl:Class rdf:about="http://ontology.inrae.fr/ppdo/ontology/SecondaryStage78">
        <rdfs:subClassOf rdf:resource="http://ontology.inrae.fr/ppdo/ontology/TwoDigitsSecondaryGrowthStage"/>
        <skos:definition xml:lang="de">80 % der Früchte erreichen art-/sortenspezifische Größe bzw. 20 % der normalen Fruchtgröße erreicht (Quelle BBCH Monografie)</skos:definition>
        <skos:definition xml:lang="fr">80% des fruits ont atteint leur taille maximale ou les fruits atteignent 80% de leur taille finale  (source BBCH monographie)</skos:definition>
        <skos:definition xml:lang="en">80% of fruits have reached final size or fruit has reached 80% of final size  (source BBCH monograph)</skos:definition>
        <skos:definition xml:lang="es">El 80% de los frutos alcanzan el tamaño especifico de su especie / variedad o bien el 80% del tamaño final (fuente BBCH monografia)</skos:definition>
        <skos:prefLabel xml:lang="de">Mikrostadium 78</skos:prefLabel>
        <skos:prefLabel xml:lang="es">estadio secondario 78</skos:prefLabel>
        <skos:prefLabel xml:lang="en">secondary stage 78</skos:prefLabel>
        <skos:prefLabel xml:lang="fr">stade secondaire 78</skos:prefLabel>
    </owl:Class>
    


    <!-- http://ontology.inrae.fr/ppdo/ontology/SecondaryStage79 -->

    <owl:Class rdf:about="http://ontology.inrae.fr/ppdo/ontology/SecondaryStage79">
        <rdfs:subClassOf rdf:resource="http://ontology.inrae.fr/ppdo/ontology/TwoDigitsSecondaryGrowthStage"/>
        <skos:definition xml:lang="es">Los frutos han alcanzado el tamaño propio de su especie / variedad (fuente BBCH monografia)</skos:definition>
        <skos:definition xml:lang="en">Nearly all fruits have reached final size  (source BBCH monograph)</skos:definition>
        <skos:definition xml:lang="de">nahezu alle Früchte erreichen art-/sortenspezifische Fruchtgröße (Quelle BBCH Monografie)</skos:definition>
        <skos:definition xml:lang="fr">presque tous les fruits ont atteint leur taille finale  (source BBCH monographie)</skos:definition>
        <skos:prefLabel xml:lang="de">Mikrostadium 79</skos:prefLabel>
        <skos:prefLabel xml:lang="es">estadio secondario 79</skos:prefLabel>
        <skos:prefLabel xml:lang="en">secondary stage 79</skos:prefLabel>
        <skos:prefLabel xml:lang="fr">stade secondaire 79</skos:prefLabel>
    </owl:Class>
    


    <!-- http://ontology.inrae.fr/ppdo/ontology/SecondaryStage81 -->

    <owl:Class rdf:about="http://ontology.inrae.fr/ppdo/ontology/SecondaryStage81">
        <rdfs:subClassOf rdf:resource="http://ontology.inrae.fr/ppdo/ontology/TwoDigitsSecondaryGrowthStage"/>
        <skos:definition xml:lang="de">Beginn der Reife bzw. Fruchtausfärbung (Quelle BBCH Monografie)</skos:definition>
        <skos:definition xml:lang="en">Beginning of ripening or fruit colouration (source BBCH monograph)</skos:definition>
        <skos:definition xml:lang="es">Comienzo de la maduración o coloración de frutos (fuente BBCH monografia)</skos:definition>
        <skos:definition xml:lang="fr">début de la maturation ou de la coloration du fruit (source BBCH monographie)</skos:definition>
        <skos:prefLabel xml:lang="de">Mikrostadium 81</skos:prefLabel>
        <skos:prefLabel xml:lang="es">estadio secondario 81</skos:prefLabel>
        <skos:prefLabel xml:lang="en">secondary stage 81</skos:prefLabel>
        <skos:prefLabel xml:lang="fr">stade secondaire 81</skos:prefLabel>
    </owl:Class>
    


    <!-- http://ontology.inrae.fr/ppdo/ontology/SecondaryStage83 -->

    <owl:Class rdf:about="http://ontology.inrae.fr/ppdo/ontology/SecondaryStage83">
        <rdfs:subClassOf rdf:resource="http://ontology.inrae.fr/ppdo/ontology/TwoDigitsSecondaryGrowthStage"/>
        <skos:definition xml:lang="de">(Weinrebe) Fortschreiten der Beeren-Aufhellung (bzw. Beeren­ Verlärbung) (Quelle BBCH Monografie)</skos:definition>
        <skos:definition xml:lang="en">(grapevigne) Berries developing colour (source BBCH monograph)</skos:definition>
        <skos:definition xml:lang="es">(vid) Las bayas, brillantes (fuente BBCH monografia)</skos:definition>
        <skos:definition xml:lang="fr">(vigne) éclaircissement et/ou changement de couleur en cours (source BBCH monographie)</skos:definition>
        <skos:prefLabel xml:lang="de">Mikrostadium 83</skos:prefLabel>
        <skos:prefLabel xml:lang="es">estadio secondario 83</skos:prefLabel>
        <skos:prefLabel xml:lang="en">secondary stage 83</skos:prefLabel>
        <skos:prefLabel xml:lang="fr">stade secondaire 83</skos:prefLabel>
    </owl:Class>
    


    <!-- http://ontology.inrae.fr/ppdo/ontology/SecondaryStage85 -->

    <owl:Class rdf:about="http://ontology.inrae.fr/ppdo/ontology/SecondaryStage85">
        <rdfs:subClassOf rdf:resource="http://ontology.inrae.fr/ppdo/ontology/TwoDigitsSecondaryGrowthStage"/>
        <skos:definition xml:lang="en">Advanced ripening or fruit colouration, (G) Dough stage (source BBCH monograph)</skos:definition>
        <skos:definition xml:lang="es">Continuación de la coloración de frutos según su especie / variedad, (G) Grano semiduro (madurez pastosa) (fuente BBCH monografia)</skos:definition>
        <skos:definition xml:lang="de">Fortschreiten der art-/sortentypischen Fruchtausfärbung, (G) Teigreife, Korninhalt noch weich, aber trocken (Quelle BBCH Monografie)</skos:definition>
        <skos:definition xml:lang="fr">stade avancé de la maturation ou de la coloration du fruit, (G) stade pâteux du caryopse  (source BBCH monographie)</skos:definition>
        <skos:prefLabel xml:lang="de">Mikrostadium 85</skos:prefLabel>
        <skos:prefLabel xml:lang="es">estadio secondario 85</skos:prefLabel>
        <skos:prefLabel xml:lang="en">secondary stage 85</skos:prefLabel>
        <skos:prefLabel xml:lang="fr">stade secondaire 85</skos:prefLabel>
    </owl:Class>
    


    <!-- http://ontology.inrae.fr/ppdo/ontology/SecondaryStage87 -->

    <owl:Class rdf:about="http://ontology.inrae.fr/ppdo/ontology/SecondaryStage87">
        <rdfs:subClassOf rdf:resource="http://ontology.inrae.fr/ppdo/ontology/TwoDigitsSecondaryGrowthStage"/>
        <skos:definition xml:lang="es">Disminución de la consistencia del fruto (fuente BBCH monografia)</skos:definition>
        <skos:definition xml:lang="en">Fruit begins to soften (species with fleshy fruit) (source BBCH monograph)</skos:definition>
        <skos:definition xml:lang="de">Verringerung der Fruchtfestigkeit (bei fleischigen Früchten) (Quelle BBCH Monografie)</skos:definition>
        <skos:definition xml:lang="fr">réduction de la fermeté des fruits (espèces à fruits charnus) (source BBCH monographie)</skos:definition>
        <skos:prefLabel xml:lang="de">Mikrostadium 87</skos:prefLabel>
        <skos:prefLabel xml:lang="es">estadio secondario 87</skos:prefLabel>
        <skos:prefLabel xml:lang="en">secondary stage 87</skos:prefLabel>
        <skos:prefLabel xml:lang="fr">stade secondaire 87</skos:prefLabel>
    </owl:Class>
    


    <!-- http://ontology.inrae.fr/ppdo/ontology/SecondaryStage89 -->

    <owl:Class rdf:about="http://ontology.inrae.fr/ppdo/ontology/SecondaryStage89">
        <rdfs:subClassOf rdf:resource="http://ontology.inrae.fr/ppdo/ontology/TwoDigitsSecondaryGrowthStage"/>
        <skos:definition xml:lang="en">Fully ripe: fruit shows fully-ripe colour, beginning of fruit abscission (source BBCH monograph)</skos:definition>
        <skos:definition xml:lang="es">Maduración plena o de recolección. Fin de la coloración típica según la especie / variedad. Los frutos o las infrutescencias se desprenden con relativa facilidad (fuente BBCH monografia)</skos:definition>
        <skos:definition xml:lang="de">Vollreiie: Art-/Sortentypische Fruchtausfärbung erreicht. Früchte bzw. Fruchtstände lösen sich relativ leicht (Quelle BBCH Monografie)</skos:definition>
        <skos:definition xml:lang="fr">la maturation ou la coloration du fruit est complète, les fruits se détachent relativement bien (source BBCH monographie)</skos:definition>
        <skos:prefLabel xml:lang="de">Mikrostadium 89</skos:prefLabel>
        <skos:prefLabel xml:lang="es">estadio secondario 89</skos:prefLabel>
        <skos:prefLabel xml:lang="en">secondary stage 89</skos:prefLabel>
        <skos:prefLabel xml:lang="fr">stade secondaire 89</skos:prefLabel>
    </owl:Class>
    


    <!-- http://ontology.inrae.fr/ppdo/ontology/SecondaryStage91 -->

    <owl:Class rdf:about="http://ontology.inrae.fr/ppdo/ontology/SecondaryStage91">
        <rdfs:subClassOf rdf:resource="http://ontology.inrae.fr/ppdo/ontology/TwoDigitsSecondaryGrowthStage"/>
        <skos:definition xml:lang="es">(P) Fin del crecimiento de la madera o de brotes (retoños), pero el follaje se mantiene verde (fuente BBCH monografia)</skos:definition>
        <skos:definition xml:lang="de">(P) Holz- bzw. Triebwachstum abgeschlossen, Laub aber noch grün (Quelle BBCH Monografie)</skos:definition>
        <skos:definition xml:lang="en">(P) Shoot development completed, foliage still green (source BBCH monograph)</skos:definition>
        <skos:definition xml:lang="fr">(P) le développement de la pousse de l’année est achevé, les feuilles sont toujours vertes (source BBCH monographie)</skos:definition>
        <skos:prefLabel xml:lang="de">Mikrostadium 91</skos:prefLabel>
        <skos:prefLabel xml:lang="es">estadio secondario 91</skos:prefLabel>
        <skos:prefLabel xml:lang="en">secondary stage 91</skos:prefLabel>
        <skos:prefLabel xml:lang="fr">stade secondaire 91</skos:prefLabel>
    </owl:Class>
    


    <!-- http://ontology.inrae.fr/ppdo/ontology/SecondaryStage92 -->

    <owl:Class rdf:about="http://ontology.inrae.fr/ppdo/ontology/SecondaryStage92">
        <rdfs:subClassOf rdf:resource="http://ontology.inrae.fr/ppdo/ontology/TwoDigitsSecondaryGrowthStage"/>
        <skos:definition xml:lang="de">(Weinrebe) Beginn der Laubblattverfärbung (Quelle BBCH Monografie)</skos:definition>
        <skos:definition xml:lang="en">(grapevigne) Beginning of leaf discolouration (source BBCH monograph)</skos:definition>
        <skos:definition xml:lang="es">(vid) Comienzo de la decoloración foliar (fuente BBCH monografia)</skos:definition>
        <skos:definition xml:lang="fr">(vigne) début de la coloration des feuilles (source BBCH monographie)</skos:definition>
        <skos:prefLabel xml:lang="de">Mikrostadium 92</skos:prefLabel>
        <skos:prefLabel xml:lang="es">estadio secondario 92</skos:prefLabel>
        <skos:prefLabel xml:lang="en">secondary stage 92</skos:prefLabel>
        <skos:prefLabel xml:lang="fr">stade secondaire 92</skos:prefLabel>
    </owl:Class>
    


    <!-- http://ontology.inrae.fr/ppdo/ontology/SecondaryStage93 -->

    <owl:Class rdf:about="http://ontology.inrae.fr/ppdo/ontology/SecondaryStage93">
        <rdfs:subClassOf rdf:resource="http://ontology.inrae.fr/ppdo/ontology/TwoDigitsSecondaryGrowthStage"/>
        <skos:definition xml:lang="de">Beginn der Blattverfärbung oder des Blattfalles (Quelle BBCH Monografie)</skos:definition>
        <skos:definition xml:lang="en">Beginning of leaf-fall (source BBCH monograph)</skos:definition>
        <skos:definition xml:lang="es">Comienzo de la decoloración o caída de las hojas (fuente BBCH monografia)</skos:definition>
        <skos:definition xml:lang="fr">début de la chute des feuilles (source BBCH monographie)</skos:definition>
        <skos:prefLabel xml:lang="de">Mikrostadium 93</skos:prefLabel>
        <skos:prefLabel xml:lang="es">estadio secondario 93</skos:prefLabel>
        <skos:prefLabel xml:lang="en">secondary stage 93</skos:prefLabel>
        <skos:prefLabel xml:lang="fr">stade secondaire 93</skos:prefLabel>
    </owl:Class>
    


    <!-- http://ontology.inrae.fr/ppdo/ontology/SecondaryStage95 -->

    <owl:Class rdf:about="http://ontology.inrae.fr/ppdo/ontology/SecondaryStage95">
        <rdfs:subClassOf rdf:resource="http://ontology.inrae.fr/ppdo/ontology/TwoDigitsSecondaryGrowthStage"/>
        <skos:definition xml:lang="es">50% de las hojas decoloradas o caídas (fuente BBCH monografia)</skos:definition>
        <skos:definition xml:lang="de">50% der Blätter verfärbt oder abgefallen (Quelle BBCH Monografie)</skos:definition>
        <skos:definition xml:lang="fr">50% des feuilles sont tombées (source BBCH monographie)</skos:definition>
        <skos:definition xml:lang="en">50% of leaves fallen (source BBCH monograph)</skos:definition>
        <skos:prefLabel xml:lang="de">Mikrostadium 95</skos:prefLabel>
        <skos:prefLabel xml:lang="es">estadio secondario 95</skos:prefLabel>
        <skos:prefLabel xml:lang="en">secondary stage 95</skos:prefLabel>
        <skos:prefLabel xml:lang="fr">stade secondaire 95</skos:prefLabel>
    </owl:Class>
    


    <!-- http://ontology.inrae.fr/ppdo/ontology/SecondaryStage97 -->

    <owl:Class rdf:about="http://ontology.inrae.fr/ppdo/ontology/SecondaryStage97">
        <rdfs:subClassOf rdf:resource="http://ontology.inrae.fr/ppdo/ontology/TwoDigitsSecondaryGrowthStage"/>
        <skos:definition xml:lang="en">End of leaf fall, plants or above ground parts dead or dormant, (P) Plant resting or dormant (source BBCH monograph)</skos:definition>
        <skos:definition xml:lang="de">Ende des Blattfalles. Pflanze bzw. oberirdische Teile abgestorben oder im Ruhestadium, (P) Pflanze in Winter- bzw. Vegetationsruhe (Quelle BBCH Monografie)</skos:definition>
        <skos:definition xml:lang="es">Fin de la caída de las hojas. Las plantas o las partes que sobresalen de la tierra han muerto o se encuentran en el estadio de reposo, (P) La planta esta en reposo invernal o vegetativo (fuente BBCH monografia)</skos:definition>
        <skos:definition xml:lang="fr">fin de la chute des feuilles, les parties aériennes de la plante sont mortes ou en phase de dormance, (P) phase de repos ou de dormance (source BBCH monographie)</skos:definition>
        <skos:prefLabel xml:lang="de">Mikrostadium 97</skos:prefLabel>
        <skos:prefLabel xml:lang="es">estadio secondario 97</skos:prefLabel>
        <skos:prefLabel xml:lang="en">secondary stage 97</skos:prefLabel>
        <skos:prefLabel xml:lang="fr">stade secondaire 97</skos:prefLabel>
    </owl:Class>
    


    <!-- http://ontology.inrae.fr/ppdo/ontology/SecondaryStage99 -->

    <owl:Class rdf:about="http://ontology.inrae.fr/ppdo/ontology/SecondaryStage99">
        <rdfs:subClassOf rdf:resource="http://ontology.inrae.fr/ppdo/ontology/TwoDigitsSecondaryGrowthStage"/>
        <skos:definition xml:lang="de">Erntegut (Stadium für die Nacherntebehandlung) (Quelle BBCH Monografie)</skos:definition>
        <skos:definition xml:lang="en">Harvested product (post-harvest or storage treatment is applied at stage 99) (source BBCH monograph)</skos:definition>
        <skos:definition xml:lang="es">Partes cosechadas (estadio para señalar tratamientos en postcosecha) (fuente BBCH monografia)</skos:definition>
        <skos:definition xml:lang="fr">produit après récolte (les traitements après la récolte ou les traitements de stockage sont appliqués) (source BBCH monographie)</skos:definition>
        <skos:prefLabel xml:lang="de">Mikrostadium 99</skos:prefLabel>
        <skos:prefLabel xml:lang="es">estadio secondario 99</skos:prefLabel>
        <skos:prefLabel xml:lang="en">secondary stage 99</skos:prefLabel>
        <skos:prefLabel xml:lang="fr">stade secondaire 99</skos:prefLabel>
    </owl:Class>
    


    <!-- http://ontology.inrae.fr/ppdo/ontology/StageDivision -->

    <owl:Class rdf:about="http://ontology.inrae.fr/ppdo/ontology/StageDivision">
        <skos:definition xml:lang="en">BBCH scale divide growth stages into principal and secondary stages. When the secondary stage is composed of three digits, the secondary digit represent an intermediary stage (source BBCH monograph)</skos:definition>
        <skos:definition xml:lang="fr">L&apos;échelle BBCH divise les stades de développement en stades principaux et secondaires. Dans le cas ou le stade secondaire est composé de 3 chiffres, le chiffre du milieu représente un stade intermédiare) (source BBCH monographie)</skos:definition>
        <skos:prefLabel xml:lang="fr">division des stades de développement d&apos;après l&apos;échelle BBCH</skos:prefLabel>
        <skos:prefLabel xml:lang="en">division of growth stages from BBCH scale</skos:prefLabel>
    </owl:Class>
    


    <!-- http://ontology.inrae.fr/ppdo/ontology/ThreeDigitsSecondaryGrowthStage -->

    <owl:Class rdf:about="http://ontology.inrae.fr/ppdo/ontology/ThreeDigitsSecondaryGrowthStage">
        <rdfs:subClassOf rdf:resource="http://ontology.inrae.fr/ppdo/ontology/SecondaryGrowthStage"/>
        <skos:definition xml:lang="es">El código de 2 dígitos es una escala que ofrece la posibilidad de precisar y definir todos los estadios fenológicos para la mayoría de las especies de plantas. Sólo en algunos casos (ej. pepino, cebolla, papa, tomate) se necesita una subdivisión más detallada junto a un estadio principal de crecimiento que vaya más allá de las posibilidades de uso de los estadios secundarios del 0 al 9. 
Para estos casos se presenta una escala de 3 dígitos al lado de la escala de 2 dígitos. Esto implica la inclusión de los también llamados mesoestadios entre los estadios principales y secundarios, que da origen a una subdivisión ampliada. Los mesoestadios 0 y 1 describen el tallo principal y los mesoestadios 2 al 9 describen los brotes laterales de 2o a 9o orden. En este caso se pueden contar hasta 19 hojas del tallo principal y además existe la posibilidad de describir las ramificaciones de las plantas.
(fuente BBCH monografia)</skos:definition>
        <skos:definition xml:lang="de">Für die Mehrzahl der Pflanzenarten wird mit dem zweistelligen Code eine Skala angeboten, die eine präzise Erfassung aller phänologischen Entwicklungsstadien ermöglicht. Lediglich bei einigen Pflanzenarten (z.B. Kartoffeln, Tomaten, Gurken und Zwiebeln) kann es notwendig sein, innerhalb eines Makrostadiums eine weitere Unterteilung vorzunehmen, als es durch die Verwendung der Mikrostadien von O bis 9 möglich ist.
Für diese Fälle wird neben der zweistelligen auch eine dreistellige Skala vorgestellt. Dabei erfolgt mit dem sogenannten Mesostadium, das zwischen Makro- und Mikrostadium eingeführt wird, eine weitere Unterteilung in der Weise, daß mit den Ziffern O und 1 das Entwicklungsgeschehen am Hauptsproß und mit den Ziffern 2
bis 9 das der Seitensprosse 2. bis 9. Ordnung be_schrieben wird. So können am Hauptsproß bis zu 19 Blätter gezählt oder das Verzweigungsgeschehen beschrieben werden.
(Quelle BBCH monografie)</skos:definition>
        <skos:definition xml:lang="fr">L’échelle de codification à 2 chiffres permet pour la plupart des espèces une description précise du stade phénologique. Néanmoins il peut être nécessaire pour certaines espèces (par exemple: pomme de terre, tomate, soja, concombre et oignon) d’introduire des codes intermédiaires qui subdivisent une nouvelle fois les stades principaux. Ainsi nous obtenons à côté des codes à 2 chiffres des codes à 3 chiffres. Le stade intermédiaire s’insérant entre le stade principal et le stade secondaire. On utilise les chiffres 0 et 1 pour la description de la tige principale, les chiffres de 2 à 9 correspondent aux pousses secondaires. Ceci permet de compter sur la tige principale jusqu’à 19 feuilles ou de décrire les pousses latérales.
(source BBCH monographie)</skos:definition>
        <skos:definition xml:lang="en">The two-digit code is a scale which offers the possibility of precisely defining all phenological growth stages for the majority of plant species. Only in the case of some plant species (e.g. cucumber, onion, potato, soybean, tomato) is further subdivision necessary within a principal growth stage beyond that possible using the secondary stages from 0 to 9. For these cases a three-digit scale is presented alongside the two-digit scale. This involves the inclusion of the so-called mesostage between the principal and the secondary stage, which provides a further subdivision... In this way up to 19 leaves can be counted on the main stem or the branching can be described.
(source BBCH monograph)</skos:definition>
    </owl:Class>
    


    <!-- http://ontology.inrae.fr/ppdo/ontology/TwoDigitsSecondaryGrowthStage -->

    <owl:Class rdf:about="http://ontology.inrae.fr/ppdo/ontology/TwoDigitsSecondaryGrowthStage">
        <rdfs:subClassOf rdf:resource="http://ontology.inrae.fr/ppdo/ontology/SecondaryGrowthStage"/>
        <skos:definition xml:lang="es">El código de 2 dígitos es una escala que ofrece la posibilidad de precisar y definir todos los estadios fenológicos para la mayoría de las especies de plantas. Sólo en algunos casos (ej. pepino, cebolla, papa, tomate) se necesita una subdivisión más detallada junto a un estadio principal de crecimiento que vaya más allá de las posibilidades de uso de los estadios secundarios del 0 al 9. 
Para estos casos se presenta una escala de 3 dígitos al lado de la escala de 2 dígitos. Esto implica la inclusión de los también llamados mesoestadios entre los estadios principales y secundarios, que da origen a una subdivisión ampliada. Los mesoestadios 0 y 1 describen el tallo principal y los mesoestadios 2 al 9 describen los brotes laterales de 2o a 9o orden. En este caso se pueden contar hasta 19 hojas del tallo principal y además existe la posibilidad de describir las ramificaciones de las plantas.
(fuente BBCH monografia)</skos:definition>
        <skos:definition xml:lang="de">Für die Mehrzahl der Pflanzenarten wird mit dem zweistelligen Code eine Skala angeboten, die eine präzise Erfassung aller phänologischen Entwicklungsstadien ermöglicht. Lediglich bei einigen Pflanzenarten (z.B. Kartoffeln, Tomaten, Gurken und Zwiebeln) kann es notwendig sein, innerhalb eines Makrostadiums eine weitere Unterteilung vorzunehmen, als es durch die Verwendung der Mikrostadien von O bis 9 möglich ist.
Für diese Fälle wird neben der zweistelligen auch eine dreistellige Skala vorgestellt. Dabei erfolgt mit dem sogenannten Mesostadium, das zwischen Makro- und Mikrostadium eingeführt wird, eine weitere Unterteilung in der Weise, daß mit den Ziffern O und 1 das Entwicklungsgeschehen am Hauptsproß und mit den Ziffern 2
bis 9 das der Seitensprosse 2. bis 9. Ordnung be_schrieben wird. So können am Hauptsproß bis zu 19 Blätter gezählt oder das Verzweigungsgeschehen beschrieben werden.
(Quelle BBCH monografie)</skos:definition>
        <skos:definition xml:lang="fr">L’échelle de codification à 2 chiffres permet pour la plupart des espèces une description précise du stade phénologique. Néanmoins il peut être nécessaire pour certaines espèces (par exemple: pomme de terre, tomate, soja, concombre et oignon) d’introduire des codes intermédiaires qui subdivisent une nouvelle fois les stades principaux. Ainsi nous obtenons à côté des codes à 2 chiffres des codes à 3 chiffres. Le stade intermédiaire s’insérant entre le stade principal et le stade secondaire. On utilise les chiffres 0 et 1 pour la description de la tige principale, les chiffres de 2 à 9 correspondent aux pousses secondaires. Ceci permet de compter sur la tige principale jusqu’à 19 feuilles ou de décrire les pousses latérales.
(source BBCH monographie)</skos:definition>
        <skos:definition xml:lang="en">The two-digit code is a scale which offers the possibility of precisely defining all phenological growth stages for the majority of plant species. Only in the case of some plant species (e.g. cucumber, onion, potato, soybean, tomato) is further subdivision necessary within a principal growth stage beyond that possible using the secondary stages from 0 to 9. For these cases a three-digit scale is presented alongside the two-digit scale. This involves the inclusion of the so-called mesostage between the principal and the secondary stage, which provides a further subdivision... In this way up to 19 leaves can be counted on the main stem or the branching can be described.
(source BBCH monograph)</skos:definition>
    </owl:Class>
    


    <!-- 
    ///////////////////////////////////////////////////////////////////////////////////////
    //
    // Individuals
    //
    ///////////////////////////////////////////////////////////////////////////////////////
     -->

    


    <!-- http://ontology.inrae.fr/ppdo/ontology/intermediary -->

    <owl:NamedIndividual rdf:about="http://ontology.inrae.fr/ppdo/ontology/intermediary">
        <rdf:type rdf:resource="http://ontology.inrae.fr/ppdo/ontology/StageDivision"/>
        <skos:definition xml:lang="en">rank of the intermediary stages</skos:definition>
    </owl:NamedIndividual>
    


    <!-- http://ontology.inrae.fr/ppdo/ontology/principal -->

    <owl:NamedIndividual rdf:about="http://ontology.inrae.fr/ppdo/ontology/principal">
        <rdf:type rdf:resource="http://ontology.inrae.fr/ppdo/ontology/StageDivision"/>
        <skos:definition xml:lang="en">rank of the principal growth stages</skos:definition>
    </owl:NamedIndividual>
    


    <!-- http://ontology.inrae.fr/ppdo/ontology/secondary -->

    <owl:NamedIndividual rdf:about="http://ontology.inrae.fr/ppdo/ontology/secondary">
        <rdf:type rdf:resource="http://ontology.inrae.fr/ppdo/ontology/StageDivision"/>
        <skos:definition xml:lang="en">rank of the secondary growth stages</skos:definition>
    </owl:NamedIndividual>
</rdf:RDF>



<!-- Generated by the OWL API (version 4.5.9.2019-02-01T07:24:44Z) https://github.com/owlcs/owlapi -->

